Proof of BDD & CP
- Work on the BDD interface, that makes it possible to prove the CP
  correct. In particular, using infinite environments was not amenable
  to prove the correctness of CP. Indeed, in CP the environment is a
  list, and that this list must be padded with values when used to
  compute the semantics of the BDD. It turned out that proving that
  the semantics was unchanged when the environment changed needed a
  huge refactor of the BDD interface.

- Work on CSE, to make it cleaner (WIP). In particular, moved the "t"
  tactic to Common.injectT, and brought back inject (as a shortcut for
  the dreadful injection foo)

- Using type classes to define the invariant led to a buggy situation
  in which it was impossible to use the exact proof term for a goal,
  because Coq tried to use type-classes inference first. SHould try to
  report a bug on that.

- Make the extraction work using Separate Extraction to avoid
  extracting the body of lemmas.

src/BDD.v
@@ -338,16 +338,18 @@ Section t.
     
     Definition mk_var bdd x :=
       mk_node bdd F x T. 
+    
+    Definition ite bdd n c l r:=
+      do cl, bdd  <- andb bdd n c l;
+      do nc, bdd  <- negb bdd n c;
+      do ncr, bdd <- andb bdd n nc r;
+      orb bdd n cl ncr.
+    
   End operations.
   
   
   (** This is the base inductive that defines the value that is
-  associated to any expression within the [bdd]. 
-
-  With hindsight, we could have defined a predicate of type bdd ->
-  expr -> Prop, that only define the shape of the (possible)
-  recursive calls, and use it as the basis to define all subsequent
-  recursion. *)
+  associated to any expression within the [bdd]. *)
 
   Inductive value bdd : expr -> bool -> Type :=
   | value_F : value bdd F false
@@ -399,12 +401,31 @@ Section t.
   Qed. 
 End t. 
 
+
+Inductive path bdd : expr -> Type :=
+| path_F : path bdd F
+| path_T : path bdd T
+| path_N : forall p l v h, 
+             PMap.find p (tmap bdd) = Some (l,v,h) -> 
+             path bdd l -> 
+             path bdd h -> 
+             path bdd (N p). 
+
+Inductive depth bdd : expr -> nat -> Type  :=
+| depth_F : forall n, depth bdd F n
+| depth_T : forall n, depth bdd T n
+| depth_N : forall n p l v h, 
+              PMap.find p (tmap bdd) = Some (l,v,h) -> 
+              depth bdd l n -> 
+              depth bdd h n -> 
+              depth bdd (N p) (S n).  
+
 (** Our bdds are well-formed, according to the following
 definition. As was hinted at before, we could have used another
 invariant here (making the acyclicity/well-foundedness more
 explicit). *)
 
-Record wf (env : nat -> bool) (b: BDD) : Type :=
+Class wf (b: BDD) : Type :=
   {
     wf_bijection : forall p n, NMap.find n (hmap b) = Some p 
                           <-> PMap.find p (tmap b) = Some n;
@@ -412,15 +433,13 @@ Record wf (env : nat -> bool) (b: BDD) : Type :=
                         (p < next b)%positive;
     wf_lt_next_find : forall p, (p < next b)%positive ->
                         {x : node | PMap.find p (tmap b) = Some x};                         
-    wf_depth : nat;
-    wf_value_interp: forall x vx, value env b x vx -> 
-                             interp env b wf_depth x = Some vx;
-    wf_value_order x vx : value env b x vx -> 
-                          forall y, order b x y ->
-                               {vy : bool & value env b y vy};
-    wf_find_value : forall p x, PMap.find p (tmap b) = Some x -> 
-                           {vp : bool & value env b (N p) vp}
-                             
+    (* wf_depth : nat; *)
+
+    (* path is a correct and complete caracterisation of the elements that are in the BDD *)
+    
+    wf_lt_path: forall p, (p < next b)%positive ->  path b (N p); 
+    wf_path_lt: forall p, path b (N p) -> (p < next b)%positive
+    (* wf_path_depth : forall p (path_p: path b p), depth b p wf_depth *)
   }.
    
 Hint Constructors value. 
@@ -443,22 +462,22 @@ Qed.
 
 Hint Resolve pmap_order_left pmap_order_right. 
 
-Record incr env (b1 b2 : BDD) :=
+Class incr (b1 b2 : BDD) :=
   {
+    incr_map: forall p x, PMap.find p (tmap b1) = Some x -> PMap.find p (tmap b2) = Some x;
     incr_order : forall x y, order b1 x y -> order b2 x y;
-    incr_value : forall x v, value env b1 x v -> 
-                            value env b2 x v;
-    incr_wf : wf env b1 -> wf env b2 
+    incr_path : forall x, path b1 x -> path b2 x;
+    incr_wf : wf b1 -> wf b2 
   }.
 
-Hint Resolve incr_value incr_order incr_wf. 
+Hint Resolve incr_path incr_order incr_wf. 
   
-Lemma incr_refl env bdd : incr env bdd bdd. 
+Lemma incr_refl bdd : incr bdd bdd. 
 Proof. 
   constructor; tauto. 
 Qed. 
 
-Lemma incr_trans env a b c : incr env a b -> incr env b c -> incr env a c. 
+Lemma incr_trans  a b c : incr a b -> incr b c -> incr a c. 
 Proof. 
   intros Hab Hbc. 
   constructor; 
@@ -466,7 +485,6 @@ Proof.
 Qed. 
 
 Hint Resolve incr_trans incr_refl. 
-
 
 Lemma interp_S n: 
   forall {env bdd p x}, 
@@ -501,12 +519,12 @@ Qed.
 
 Hint Resolve interp_S. 
 
-Lemma value_upd  env bdd (Hwf: wf env bdd) l v h:
+Lemma value_upd  env bdd (Hwf: wf bdd) l v h:
   NMap.find (l,v,h) (hmap bdd) = None ->
   forall vl, value env bdd l vl -> 
-        forall vh, value env bdd h vh -> 
-              forall x vx, value env bdd x vx -> 
-                      value env (upd bdd (l,v,h)) x vx. 
+  forall vh, value env bdd h vh -> 
+  forall x vx, value env bdd x vx -> 
+          value env (upd bdd (l,v,h)) x vx. 
 Proof.              
   intros Hbdd vl Hvl vh Hvh x vx H.
   induction H. 
@@ -517,6 +535,23 @@ Proof.
   destruct Hwf as [ _ Hwf]. apply Hwf in e. clear - e. zify; omega. 
 Qed. 
 Hint Resolve value_upd.   
+
+Lemma path_upd  bdd (Hwf: wf bdd) l v h:
+  NMap.find (l,v,h) (hmap bdd) = None ->
+  path bdd l -> 
+  path bdd h -> 
+  forall x, path bdd x  -> 
+  path (upd bdd (l,v,h)) x. 
+Proof.              
+  intros Hbdd Hvl Hvh x H.
+  induction H. 
+  constructor. 
+  constructor. 
+  apply (path_N _ _ l0 v0 h0); auto. 
+  simpl. rewrite PMap.gso. apply e.
+  destruct Hwf as [ _ Hwf]. apply Hwf in e. clear - e. zify; omega. 
+Qed. 
+Hint Resolve path_upd.   
 
 Lemma expr_eq_dec (e1 e2: expr) : ({e1 = e2} + {e1 <> e2})%type.  
 Proof.
@@ -568,31 +603,55 @@ Proof.
   apply expr_compare_eq in H1. apply expr_compare_eq in H3. subst; reflexivity.
 Qed. 
 
-Remark wf_neq env bdd (Hwf : wf env bdd) p x : PMap.find p (tmap bdd) = Some x -> p <> next bdd. 
+Remark wf_neq bdd (Hwf : wf bdd) p x : PMap.find p (tmap bdd) = Some x -> p <> next bdd. 
 Proof. 
-  intros H. apply (wf_lt_next _ _ Hwf) in H; auto.  zify; omega. 
+  intros H. apply (wf_lt_next)  in H; auto.  zify; omega. 
 Qed. 
 Hint Resolve wf_neq. 
-  
 
+
+(* Lemma value_upd_inj x vx vy : value env bdd x vx ->  *)
+(*                               value env (upd bdd (l,v,h)) x vy ->  *)
+(*                               vx = vy.  *)
+(* Proof. *)
+(*   intros.  *)
+(*   eapply value_upd in H; eauto.  *)
+(* Qed.  *)
+      
+Lemma order_path bdd x y : path bdd x -> order bdd x y -> path bdd y. 
+Proof. 
+  intros. 
+  inversion H; subst. 
+  compute in X; intuition; discriminate. 
+  compute in X; intuition; discriminate.
+  unfold order in X. destruct X. simpl in e. rewrite H0 in e. injection e; intros; subst. auto. 
+  simpl in e. rewrite H0 in e. injection e; intros; subst. auto. 
+Qed. 
+  
 Section wf_upd.  
-  Variable env : nat -> bool. 
   Variable bdd : BDD. 
-  Hypothesis Hwf : wf env bdd.
+  Hypothesis Hwf : wf bdd.
   Variable (l:expr) (v:nat) (h:expr). 
-  Variable vl vh : bool. 
-  Hypothesis Hvl : value env bdd l vl. 
-  Hypothesis Hvh : value env bdd h vh. 
+  Hypothesis Hvl : path bdd l. 
+  Hypothesis Hvh : path bdd h. 
   Hypothesis Hnode : NMap.find (elt:=positive) (l, v, h) (hmap bdd) = None.
 
-  Remark value_upd_left : value env (upd bdd (l,v,h)) l vl. 
-  Proof. 
-    eapply value_upd; eauto. 
-  Qed. 
-  Remark value_upd_right : value env (upd bdd (l,v,h)) h vh. 
-  Proof. 
-    eapply value_upd; eauto. 
-  Qed. 
+  (* Remark value_upd_left : value env (upd bdd (l,v,h)) l vl.  *)
+  (* Proof.  *)
+  (*   eapply value_upd; eauto.  *)
+  (* Qed.  *)
+  (* Remark value_upd_right : value env (upd bdd (l,v,h)) h vh.  *)
+  (* Proof.  *)
+  (*   eapply value_upd; eauto.  *)
+  (* Qed.  *)
+  Remark path_upd_left :  path  (upd bdd (l,v,h)) l.
+  Proof.
+    eapply path_upd; eauto.
+  Qed.
+  Remark path_upd_right : path (upd bdd (l,v,h)) h.
+  Proof.
+    eapply path_upd; eauto.
+  Qed.
   
   Lemma order_upd : forall x y : expr, order bdd x y -> order (upd bdd (l, v, h)) x y.
   Proof. 
@@ -609,15 +668,7 @@ Section wf_upd.
        * rewrite H in Hxy. discriminate.
   Qed.  
          
-  Lemma value_upd_inj x vx vy : value env bdd x vx -> 
-                        value env (upd bdd (l,v,h)) x vy -> 
-                        vx = vy. 
-  Proof.
-    intros. 
-    eapply value_upd in H; eauto. 
-  Qed. 
-    
-  Lemma interp_upd : forall (n : var) (x : expr) (y : bool),
+  Lemma interp_upd env : forall (n : var) (x : expr) (y : bool),
                        interp env bdd n x = Some y -> interp env (upd bdd (l, v, h)) n x = Some y.
   Proof.
     induction n; intros. discriminate.
@@ -629,48 +680,72 @@ Section wf_upd.
     destruct (env v2) eqn: Heq;t; intuition.
   Qed.
     
-  Lemma wf_value_lt x vx : value env bdd (N x) vx -> 
+  Lemma wf_value_lt env x vx : value env bdd (N x) vx -> 
                            (x < next bdd)%positive. 
   Proof.
     clear - Hwf. 
     intros H. inversion H.  subst.
-    apply (wf_lt_next _ _ Hwf) in H1. auto. 
+    apply (wf_lt_next) in H1. auto. 
   Qed. 
   
-  Hint Resolve wf_value_lt wf_value_order.
+  Hint Resolve wf_value_lt.
+  Hint Resolve wf_path_lt.
+  (* Lemma value_upd_neq x vx :  value env (upd bdd (l, v, h)) x vx -> *)
+  (*                             N (next bdd) <> x -> *)
+  (*                             value env bdd x vx. *)
+  (* Proof. *)
+  (*   intros.  *)
+  (*   induction H;  auto.  *)
+  (*   simpl in e. rewrite PMap.gso in e by congruence.  *)
+  (*   destruct (wf_find_value _ _ Hwf  _ _ e) as [vp Hvp].  *)
 
-  Lemma value_upd_neq x vx :  value env (upd bdd (l, v, h)) x vx ->
+  (*   refine (let IH1 := IHvalue1 _ in  *)
+  (*           let IH2 := IHvalue2 _ in _).  *)
+  (*   destruct l0 as [ | | X ]; try discriminate;   *)
+  (*   assert (HX : (X < next bdd)%positive) by *)
+  (*       (refine (let H := wf_value_order _ _ Hwf _ _ Hvp  (N X) _ in  *)
+  (*                let (x, Hx) := H in wf_value_lt _ _ Hx  *)
+  (*              ); [eauto ]).  *)
+  (*   clear - HX. intros H; injection H; clear H. zify; omega.  *)
+  (*   destruct h0 as [ | | X ]; try discriminate;   *)
+  (*   assert (HX : (X < next bdd)%positive) by *)
+  (*       (refine (let H := wf_value_order _ _ Hwf _ _ Hvp  (N X) _ in  *)
+  (*                let (x, Hx) := H in wf_value_lt _ _ Hx  *)
+  (*              ); [eauto ]).  *)
+  (*   clear - HX. intros H; injection H; clear H; intros. zify; omega.  *)
+  (*   econstructor; eauto.  *)
+  (* Qed. *)
+  
+  Hint Constructors path. 
+
+  Lemma path_upd_neq x :  path (upd bdd (l, v, h)) x  ->
                               N (next bdd) <> x ->
-                              value env bdd x vx.
-  Proof.
-    intros. 
-    induction H;  auto. 
-    simpl in e. rewrite PMap.gso in e by congruence. 
-    destruct (wf_find_value _ _ Hwf  _ _ e) as [vp Hvp]. 
+                              path bdd x.
+  Proof. 
+    intros. induction H; auto. 
+    simpl in e. rewrite PMap.gso in e by congruence.
+    
+    refine (let IH1 := IHpath1 _ in
+            let IH2 := IHpath2 _ in _); clear IHpath1 IHpath2. 
+    
+    destruct l0 as [ | | X ]; try discriminate. 
+    assert (HX : (X < next bdd)%positive). 
+    eauto 6 using wf_path_lt, wf_lt_path, wf_lt_next, order_path. 
+    intros H'.  injection H'. subst.   zify. omega. 
 
-    refine (let IH1 := IHvalue1 _ in 
-            let IH2 := IHvalue2 _ in _). 
-    destruct l0 as [ | | X ]; try discriminate;  
-    assert (HX : (X < next bdd)%positive) by
-        (refine (let H := wf_value_order _ _ Hwf _ _ Hvp  (N X) _ in 
-                 let (x, Hx) := H in wf_value_lt _ _ Hx 
-               ); [eauto ]). 
-    clear - HX. intros H; injection H; clear H. zify; omega. 
-    destruct h0 as [ | | X ]; try discriminate;  
-    assert (HX : (X < next bdd)%positive) by
-        (refine (let H := wf_value_order _ _ Hwf _ _ Hvp  (N X) _ in 
-                 let (x, Hx) := H in wf_value_lt _ _ Hx 
-               ); [eauto ]). 
-    clear - HX. intros H; injection H; clear H; intros. zify; omega. 
+    destruct h0 as [ | | X ]; try discriminate. 
+    assert (HX : (X < next bdd)%positive). 
+    eauto 6 using wf_path_lt, wf_lt_path, wf_lt_next, order_path. 
+    intros H'.  injection H'. subst.   zify. omega. 
+
     econstructor; eauto. 
   Qed.
-
   
   (* Lemma value_upd_eq x vx : value env (upd bdd (l,v,h)) x vx -> *)
   (*                           x = N (next bdd) ->  *)
   (*                           value env (upd bdd (l,v,h)) x (if env v then vh else vl).  *)
   
-  Lemma order_upd_eq x y : order (upd bdd (l,v,h)) x y -> 
+  Lemma order_upd_eq env x y : order (upd bdd (l,v,h)) x y -> 
                            x = N (next bdd) -> 
                            forall vx, value env (upd bdd (l,v,h)) x vx ->
                                  (y = l) + (y = h). 
@@ -684,7 +759,7 @@ Section wf_upd.
     right; congruence. 
   Qed. 
   
-  Lemma order_upd_neq x y : order (upd bdd (l,v,h)) x y -> 
+  Lemma order_upd_neq env x y : order (upd bdd (l,v,h)) x y -> 
                             x <> N (next bdd) -> 
                             forall vx, value env (upd bdd (l,v,h)) x vx ->
                                   order bdd x y. 
@@ -698,17 +773,9 @@ Section wf_upd.
     right; apply H. 
   Qed. 
   
-  Lemma wf_upd : wf env (upd bdd (l, v, h)).
+  Lemma wf_upd : wf (upd bdd (l, v, h)).
   Proof. 
-    
-    refine ((fun wf_equiv wf_lt_next wf_depth wf_value_interp wf_value_order wf_find_value =>
-              Build_wf env _
-                       wf_equiv wf_lt_next wf_depth 
-                       wf_value_interp 
-                       (wf_value_order (* wf_find_value env wf_value_interp *))
-                       wf_find_value
-            ) _ _ _ (1 + wf_depth env _ Hwf) _ _  _). 
-
+    apply Build_wf. 
     - clear Hvl Hvh. revert Hnode.   generalize (l,v,h) as n1; intros n1 Hn1 p n2. 
       simpl. 
       destruct (node_eq_dec n1 n2) as [Hn | Hn]; [subst|].
@@ -720,25 +787,25 @@ Section wf_upd.
           destruct (Pos.eq_dec (next bdd) p); [trivial|]. 
           exfalso. 
           rewrite PMap.gso in H by congruence. 
-          rewrite <- (wf_bijection _ _ Hwf) in H; congruence. 
+          rewrite <- (wf_bijection) in H; congruence. 
         * apply node_compare_refl. 
-          
       + rewrite NMapFacts.add_neq_o by (rewrite node_compare_eq_iff; tauto).
         split; intros. 
-        rewrite (wf_bijection _ _ Hwf) in H. 
+        rewrite (wf_bijection) in H. 
         rewrite PMap.gso; eauto. 
         rewrite PMap.gso in H. 
-        rewrite (wf_bijection _ _ Hwf ); auto. 
+        rewrite (wf_bijection); auto. 
 
         intros Hp. subst. 
         rewrite PMap.gss in H. congruence. 
+
     - intros. 
       simpl in H. 
       destruct (Pos.eq_dec (next bdd) p). subst. unfold upd. unfold next at 2.  
       zify; omega. 
       unfold upd. unfold next at 1. 
       rewrite PMap.gso in H by eauto. 
-      apply (wf_lt_next _ _ Hwf) in H; zify; omega. 
+      apply (wf_lt_next) in H; zify; omega. 
     - intros. 
       {
         unfold upd in H. unfold next at 1 in H. 
@@ -746,53 +813,28 @@ Section wf_upd.
         exists (l,v,h). rewrite PMap.gss. reflexivity. 
         assert ((p < next bdd)%positive). 
         zify;omega. 
-        destruct (wf_lt_next_find env bdd Hwf _ H0) as [x Hx]. 
+        destruct (wf_lt_next_find _ H0) as [x Hx]. 
         exists x. simpl. rewrite PMap.gso by eauto. auto. 
       }
-    - intros.
-      destruct (expr_eq_dec (N (next bdd)) x). 
-      + subst; simpl. 
-        inversion H. subst. simpl in H1. 
-        pose proof Hvl. clear Hvl. 
-        pose proof Hvh. clear Hvh. 
-        
-        rewrite H1.
-        rewrite PMap.gss in H1.
-        injection H1; intros. destruct H5. destruct H6. destruct H7. simpl. 
-        simpl.                  
-        destruct (env v). 
-        * apply interp_upd. 
-          apply Hwf.
-          assert (vh = vh0). eapply value_upd_inj; eauto.  subst. eauto. 
-        *  apply interp_upd. 
-           apply Hwf.
-           assert (vl = vl0). eapply value_upd_inj; eauto.  subst. eauto. 
-      + apply interp_upd. apply interp_S. apply Hwf.
-        apply value_upd_neq; assumption.  
-    - intros.
-      
-      destruct (expr_eq_dec (N (next bdd)) x).
-      eapply order_upd_eq in X; eauto. destruct X; subst; eauto.
-      eapply order_upd_neq in X; eauto. 
-      eapply value_upd_neq in H; eauto. 
-      pose proof (wf_value_order _ _ Hwf _ _ H _ X). destruct H0 as [vy Hvy]. exists vy. eauto. 
     - intros. 
-      simpl in H. 
-      destruct (Pos.eq_dec p (next bdd)); subst. 
-      pose proof H.
-      rewrite PMap.gss in H. injection H; intros; subst; clear H. 
-      exists (if env v then vh else vl). econstructor; eauto. 
-      
-      rewrite PMap.gso in H by eassumption. apply (wf_find_value env _ Hwf) in H. destruct H.
-      eapply value_upd in v0; eauto. 
+      destruct (Pos.eq_dec (next bdd) (p)). 
+      + subst.
+        apply (path_N _ (next bdd) l v h); auto.  simpl. rewrite PMap.gss; reflexivity.
+      + apply path_upd; auto. apply wf_lt_path. unfold upd in H. unfold next at 1 in H.  zify. omega. 
+    - intros. 
+      destruct (Pos.eq_dec (next bdd) (p)). 
+      + subst. unfold upd.  unfold next at 2. zify; omega. 
+      + subst. unfold upd.  unfold next at 1. 
+        apply path_upd_neq in H.  2: congruence.  
+        apply wf_path_lt in H. zify;omega. 
   Qed. 
 End wf_upd. 
 
-Lemma mk_node_correct {env bdd} (Hwf: wf env bdd) {l v h e bdd'}: 
+Lemma mk_node_correct {env bdd} (Hwf: wf  bdd) {l v h e bdd'}: 
   mk_node bdd l v h = (e,bdd') -> 
   forall vl, value env bdd l vl -> 
   forall vh, value env bdd h vh -> 
-        (value env bdd' e (if env v then vh else vl) * incr env bdd bdd')%type.       
+        (value env bdd' e (if env v then vh else vl) * incr  bdd bdd')%type.       
 Proof. 
   intros.
   unfold mk_node in H. 
@@ -811,21 +853,30 @@ Proof.
     + rewrite Hnode in H.
       injection H; intros; subst; clear H.
       split ; [|auto]. 
-      rewrite (wf_bijection _ _ Hwf) in Hnode. econstructor; eauto. 
+      rewrite (wf_bijection ) in Hnode. econstructor; eauto. 
     + rewrite Hnode in H.
       injection H; intros; subst; clear H.
-      refine ((fun H H' => ((H' H), H)) _ _). 
-      {                       (* proof of incr *)
-        constructor. 
-        - apply (order_upd env); auto.  
-        - eapply value_upd; eauto. 
-        - intros _.
-          {
-            eapply wf_upd; eauto.  
-          }
-          
-      }
-      {
+      assert (incr bdd (upd bdd (l,v,h))). 
+      {constructor.
+       * intros. 
+         simpl. rewrite PMap.gso; auto.  
+         apply wf_lt_next in H. zify;omega.         
+       * apply (order_upd); auto.  
+       * eapply path_upd; eauto. 
+         Lemma path_of_value env bdd x vx : 
+           value env bdd x vx -> 
+           path bdd x. 
+         Proof. 
+           induction 1; try constructor. 
+           econstructor. apply e. auto.  auto. 
+         Qed. 
+         Hint Resolve path_of_value. 
+         eauto. 
+         eauto. 
+       * intros. eapply wf_upd; eauto.  
+      }      
+      
+      { split; auto. 
         intros. econstructor; 
                 [
                 | eapply value_upd; eauto
@@ -847,231 +898,715 @@ Ltac t s ::=
        | H : (bind ?x ?f = None) |- _ => 
          destruct (bind_inversion_None x f H) as [?H | [?x [?I ?I]]]
        | H : ?x = Some ?y |- context [?x] => rewrite H
-       | |- (_ * incr ?env ?x ?x)%type => refine ( _ , incr_refl env x )                              
+       | |- (_ * incr ?x ?x)%type => refine ( _ , incr_refl x )                              
        | H : value ?env ?b T _ |- _ => apply (value_T_inversion env b) in H
        | H : value ?env ?b F _ |- _ => apply (value_F_inversion env b) in H
        | |- value ?env _ T _ => constructor
        | |- value ?env _ F _ => constructor
        | |- _ => subst           
       end) || s); trivial.
+Lemma incr_value env bdd1 bdd2 x vx (Hincr:incr bdd1 bdd2) :
+  value env bdd1 x vx -> 
+  value env bdd2 x vx. 
+Proof.   
+  induction 1; try constructor. 
+  econstructor; eauto using incr_map.  
+Qed. 
 
-Section cases. 
-  Ltac inj :=
-    repeat match goal with 
-             | H : value ?env ?b ?x ?vx , H' : value ?env ?b ?x ?vy |- _ =>  
-               let H'' := fresh in 
-               assert (H'' := value_inj env b x vx H vy H'); 
-                 clear H'; subst
-           end. 
-  
-  Variables
-    (env : var -> bool)
-    (bdd : BDD)
-    (Hwf : wf env bdd)
-    (op : bool -> bool -> bool)
-    (opb: BDD -> nat -> expr -> expr -> option (expr * BDD))
-    (n : nat)
-    (IH:  forall bdd : BDD,
-            wf env bdd ->
-            forall (a b ab : expr) (bdd' : BDD),
-              opb bdd n a b = Some (ab, bdd') ->
+Hint Resolve incr_value.   
+Section value. 
+  Section binop. 
+    Ltac inj :=
+      repeat match goal with 
+               | H : value ?env ?b ?x ?vx , H' : value ?env ?b ?x ?vy |- _ =>  
+                 let H'' := fresh in 
+                 assert (H'' := value_inj env b x vx H vy H'); 
+                   clear H'; subst
+             end. 
+    
+    Variables
+      (env : var -> bool)
+      (bdd : BDD)
+      (Hwf : wf bdd)
+      (op : bool -> bool -> bool)
+      (opb: BDD -> nat -> expr -> expr -> option (expr * BDD))
+      (n : nat)
+      (IH:  forall bdd : BDD,
+              wf  bdd ->
+              forall (a b ab : expr) (bdd' : BDD),
+                opb bdd n a b = Some (ab, bdd') ->
               forall va : bool,
                 value env bdd a va ->
                 forall vb : bool,
                   value env bdd b vb ->
-                  value env bdd' ab (op va vb) * incr env bdd bdd')
-    (a b: positive)
-    (va vb: bool)
-    (Hva : value env bdd (N a) va)
-    (Hvb : value env bdd (N b) vb)
-    (la : expr) (xa: var) (ha: expr) (Ha : PMap.find a (tmap bdd) = Some (la, xa, ha))
-    (lb : expr) (xb: var) (hb: expr) (Hb : PMap.find b (tmap bdd) = Some (lb, xb, hb)).
+                  value env bdd' ab (op va vb) * incr  bdd bdd')
+      (a b: positive)
+      (va vb: bool)
+      (Hva : value env bdd (N a) va)
+      (Hvb : value env bdd (N b) vb)
+      (la : expr) (xa: var) (ha: expr) (Ha : PMap.find a (tmap bdd) = Some (la, xa, ha))
+      (lb : expr) (xb: var) (hb: expr) (Hb : PMap.find b (tmap bdd) = Some (lb, xb, hb)).
   
   
-  Lemma binop_correct_lt : forall
-                             l bdd1 (H1 : opb bdd n la (N b) = Some (l, bdd1))
-                             h bdd2 (H2 : opb bdd1 n ha (N b) = Some (h, bdd2))
-                             ab bdd3 (H3 : mk_node bdd2 l xa h = (ab, bdd3)),
-                             (value env bdd3 ab (op va vb) * incr env bdd bdd3). 
-  Proof. 
-    intros. 
-    destruct (value_N_inversion env bdd a va Hva _ _ _ Ha) as [vla [vha [[Hla Hha] Hwa]]].
-    destruct (value_N_inversion env bdd b vb Hvb _ _ _ Hb) as [vlb [vhb [[Hlb Hhb] Hwb]]].
-    destruct (IH _ Hwf _ _ _ _ H1 _ Hla _ Hwb) as [Hvx Hincr]. 
-    refine (let (Hvx1,Hincr2) := IH bdd1 (_ : wf env bdd1) _ _ _ _ H2 
-                                     _ (_: value env bdd1 ha vha) 
-                                     _ (_: value env bdd1 (N b) _) in _
-           ); eauto. 
-    inj. 
-    refine (let (Hab, Hincr2) := mk_node_correct ( _ : wf env bdd2) H3 _ _ _ _ in _
-           ); eauto. 
-    destruct (env xa); destruct (env xb); split; eauto. 
-  Qed. 
-   
-  Lemma binop_correct_gt : forall
-                             l bdd1 (H1 : opb bdd n (N a) lb  = Some (l, bdd1))
-                             h bdd2 (H2 : opb bdd1 n (N a) hb = Some (h, bdd2))
-                             ab bdd3 (H3 : mk_node bdd2 l xb h = (ab, bdd3)),
-                             (value env bdd3 ab (op va vb) * incr env bdd bdd3). 
-  Proof. 
-    intros. 
-    destruct (value_N_inversion env bdd a va Hva _ _ _ Ha) as [vla [vha [[Hla Hha] Hwa]]].
-    destruct (value_N_inversion env bdd b vb Hvb _ _ _ Hb) as [vlb [vhb [[Hlb Hhb] Hwb]]].
-    destruct (IH _ Hwf _ _ _ _ H1 _ Hwa _ Hlb) as [Hvx Hincr]. 
-    refine (let (Hvx1,Hincr2) := IH bdd1 (_ : wf env bdd1) _ _ _ _ H2 
-                                     _ (_: value env bdd1 (N a) _) 
-                                     _ (_: value env bdd1 hb vhb) in _
-           ); eauto. 
-    inj. 
-    refine (let (Hab, Hincr2) := mk_node_correct _ H3 _ _ _ _ in _
-           ); eauto. 
-    split. destruct (env xa); destruct (env xb); auto.  
-    eauto. 
-  Qed.
+    Lemma binop_correct_lt : forall
+                               l bdd1 (H1 : opb bdd n la (N b) = Some (l, bdd1))
+                               h bdd2 (H2 : opb bdd1 n ha (N b) = Some (h, bdd2))
+                               ab bdd3 (H3 : mk_node bdd2 l xa h = (ab, bdd3)),
+                               (value env bdd3 ab (op va vb) * incr  bdd bdd3). 
+    Proof. 
+      intros. 
+      destruct (value_N_inversion env bdd a va Hva _ _ _ Ha) as [vla [vha [[Hla Hha] Hwa]]].
+      destruct (value_N_inversion env bdd b vb Hvb _ _ _ Hb) as [vlb [vhb [[Hlb Hhb] Hwb]]].
+      destruct (IH _ Hwf _ _ _ _ H1 _ Hla _ Hwb) as [Hvx Hincr]. 
+      refine (let (Hvx1,Hincr2) := IH bdd1 (_ : wf  bdd1) _ _ _ _ H2 
+                                      _ (_: value env bdd1 ha vha) 
+                                      _ (_: value env bdd1 (N b) _) in _
+             ); eauto. 
+      
+      inj. 
+      refine (let (Hab, Hincr2) := mk_node_correct ( _ : wf bdd2) H3 _ _ _ _ in _
+             ); eauto. 
+      destruct (env xa); destruct (env xb); split; eauto. 
+    Qed. 
+    
+    Lemma binop_correct_gt : forall
+                               l bdd1 (H1 : opb bdd n (N a) lb  = Some (l, bdd1))
+                               h bdd2 (H2 : opb bdd1 n (N a) hb = Some (h, bdd2))
+                               ab bdd3 (H3 : mk_node bdd2 l xb h = (ab, bdd3)),
+                               (value env bdd3 ab (op va vb) * incr bdd bdd3). 
+    Proof. 
+      intros. 
+      destruct (value_N_inversion env bdd a va Hva _ _ _ Ha) as [vla [vha [[Hla Hha] Hwa]]].
+      destruct (value_N_inversion env bdd b vb Hvb _ _ _ Hb) as [vlb [vhb [[Hlb Hhb] Hwb]]].
+      destruct (IH _ Hwf _ _ _ _ H1 _ Hwa _ Hlb) as [Hvx Hincr]. 
+      refine (let (Hvx1,Hincr2) := IH bdd1 (_ : wf  bdd1) _ _ _ _ H2 
+                                      _ (_: value env bdd1 (N a) _) 
+                                      _ (_: value env bdd1 hb vhb) in _
+             ); eauto. 
+      inj. 
+      refine (let (Hab, Hincr2) := mk_node_correct _ H3 _ _ _ _ in _
+             ); eauto. 
+      split. destruct (env xa); destruct (env xb); auto.  
+      eauto. 
+    Qed.
   
-  Lemma binop_correct_eq (Heq: xa = xb) : forall
-                             l bdd1 (H1 : opb bdd n la lb  = Some (l, bdd1))
-                             h bdd2 (H2 : opb bdd1 n ha hb = Some (h, bdd2))
-                             ab bdd3 (H3 : mk_node bdd2 l xa h = (ab, bdd3)),
-                             (value env bdd3 ab (op va vb) * incr env bdd bdd3). 
-  Proof. 
-    intros. subst.  
-    destruct (value_N_inversion env bdd a va Hva _ _ _ Ha) as [vla [vha [[Hla Hha] Hwa]]].
-    destruct (value_N_inversion env bdd b vb Hvb _ _ _ Hb) as [vlb [vhb [[Hlb Hhb] Hwb]]].
-    destruct (IH _ Hwf _ _ _ _ H1 _ Hla _ Hlb) as [Hvx Hincr]. 
-    refine (let (Hvx1,Hincr2) := IH bdd1 (_ : wf env bdd1) _ _ _ _ H2 
-                                     _ (_: value env bdd1 ha vha) 
-                                     _ (_: value env bdd1 hb vhb) in _
-           ); eauto. 
-    inj. 
-    refine (let (Hab, Hincr2) := mk_node_correct _ H3 _ _ _ _ in _
-           ); eauto. 
-    split; destruct (env xb); eauto.  
-  Qed. 
-End cases. 
+    Lemma binop_correct_eq (Heq: xa = xb) : forall
+                                              l bdd1 (H1 : opb bdd n la lb  = Some (l, bdd1))
+                                              h bdd2 (H2 : opb bdd1 n ha hb = Some (h, bdd2))
+                                              ab bdd3 (H3 : mk_node bdd2 l xa h = (ab, bdd3)),
+                                              (value env bdd3 ab (op va vb) * incr bdd bdd3). 
+    Proof. 
+      intros. subst.  
+      destruct (value_N_inversion env bdd a va Hva _ _ _ Ha) as [vla [vha [[Hla Hha] Hwa]]].
+      destruct (value_N_inversion env bdd b vb Hvb _ _ _ Hb) as [vlb [vhb [[Hlb Hhb] Hwb]]].
+      destruct (IH _ Hwf _ _ _ _ H1 _ Hla _ Hlb) as [Hvx Hincr]. 
+      refine (let (Hvx1,Hincr2) := IH bdd1 (_ : wf bdd1) _ _ _ _ H2 
+                                      _ (_: value env bdd1 ha vha) 
+                                      _ (_: value env bdd1 hb vhb) in _
+             ); eauto. 
+      inj. 
+      refine (let (Hab, Hincr2) := mk_node_correct _ H3 _ _ _ _ in _
+             ); eauto. 
+      split; destruct (env xb); eauto.  
+    Qed. 
+  End binop.  
 
-Lemma andb_correct env bdd (Hwf: wf env bdd) n a b ab bdd' :
-  andb bdd n a b = Some (ab, bdd') ->
-  forall va, value env bdd a va -> 
-        forall vb, value env bdd b vb -> 
-              (value env bdd' ab (va && vb)%bool * incr env bdd bdd').
-Proof.
-  revert bdd Hwf a b ab bdd'. 
-  induction n; intros bdd Hwf a b ab bdd' Hand va Hva vb Hvb. 
-  - discriminate. 
-  - simpl in Hand. 
+  Lemma andb_correct env bdd (Hwf: wf bdd) n a b ab bdd' :
+    andb bdd n a b = Some (ab, bdd') ->
+    forall va, value env bdd a va -> 
+          forall vb, value env bdd b vb -> 
+                (value env bdd' ab (va && vb)%bool * incr bdd bdd').
+  Proof.
+    revert bdd Hwf a b ab bdd'. 
+    induction n; intros bdd Hwf a b ab bdd' Hand va Hva vb Hvb. 
+    - discriminate. 
+    - simpl in Hand. 
     Ltac s := 
       try match goal with 
-        | |- context [(_ && false)%bool]  => rewrite Bool.andb_comm; simpl Datatypes.andb
-        | |- context [(_ && true)%bool]  => rewrite Bool.andb_comm; simpl  Datatypes.andb
-        | |- context [(false && _ )%bool]  => simpl  Datatypes.andb
-        | |- context [(true  && _ )%bool]  => simpl  Datatypes.andb
-      end.  
+            | |- context [(_ && false)%bool]  => rewrite Bool.andb_comm; simpl Datatypes.andb
+            | |- context [(_ && true)%bool]  => rewrite Bool.andb_comm; simpl  Datatypes.andb
+            | |- context [(false && _ )%bool]  => simpl  Datatypes.andb
+            | |- context [(true  && _ )%bool]  => simpl  Datatypes.andb
+          end.  
     destruct a as [ | | a]; destruct b as [ | | b]; simpl in *; t s.  
+    
     destruct x as [[la xa] ha]. destruct x0 as [[lb xb] hb]. 
     destruct (NPeano.Nat.compare xa xb) eqn: Heq.
-    + apply nat_compare_eq in Heq; subst; t s. 
-      eauto using binop_correct_eq. 
-    + t s; eauto using binop_correct_lt.
-      
-    + t s; eauto using binop_correct_gt. 
-Qed.
-
-
-Lemma orb_correct env bdd (Hwf: wf env bdd) n a b ab bdd' :
-  orb bdd n a b = Some (ab, bdd') ->
-  forall va, value env bdd a va -> 
-  forall vb, value env bdd b vb -> 
-  (value env bdd' ab (va || vb)%bool * incr env bdd bdd').
-Proof.
-  revert bdd Hwf a b ab bdd'. 
-  induction n; intros bdd Hwf a b ab bdd' Hand va Hva vb Hvb. 
-  - discriminate. 
-  - simpl in Hand. 
-  Ltac s ::= 
-       try 
-       match goal with 
-        | |- context [(_ || false)%bool]  => rewrite Bool.orb_comm; simpl Datatypes.orb
-        | |- context [(_ || true)%bool]  => rewrite Bool.orb_comm; simpl  Datatypes.orb
-        | |- context [(false || _ )%bool]  => simpl  Datatypes.orb
-        | |- context [(true  || _ )%bool]  => simpl  Datatypes.orb
-       end.
-  destruct a as [ | | a]; destruct b as [ | | b]; simpl in *; t s.
-  destruct x as [[la xa] ha]. destruct x0 as [[lb xb] hb]. 
-  destruct (NPeano.Nat.compare xa xb) eqn: Heq.
-    + apply nat_compare_eq in Heq; subst; t s. 
-      eauto using binop_correct_eq. 
-    + t s; eauto using binop_correct_lt.        
-    + t s; eauto using binop_correct_gt.
-Qed.  
-
-Lemma negb_correct env bdd (Hwf: wf env bdd) n a a' bdd' :
-  negb bdd n a = Some (a', bdd') ->
-  forall va, value env bdd a va -> 
-  (value env bdd' a' (Datatypes.negb va)%bool * incr env bdd bdd').
-Proof.
-  revert bdd Hwf a a' bdd'. 
-  induction n; intros bdd Hwf a a' bdd' Hnegb va Hva. 
-  - discriminate. 
-  - simpl in Hnegb. 
-  Ltac s ::= 
-       try
-       match goal with 
-        | |- context [(Datatypes.negb false)%bool] =>  simpl Datatypes.negb 
-        | |- context [(Datatypes.negb true)%bool]  =>  simpl Datatypes.negb
-       end. 
-  destruct a as [ | | a]; simpl in *; t s.
-  destruct x as [[la xa] ha]; t s.
-  destruct (value_N_inversion env bdd a va Hva _ _ _ I) as [vla [vha [[Hla Hha] Hwa]]].
-  destruct (IHn _ Hwf _ _ _ I1 _ Hla) as [Hvx Hincr]; clear I1. 
-  refine (let (Hvx1,Hincr2) := IHn x0 (_ : wf env x0) _ _ _ I0 
-                           _ (_: value env _ ha vha) 
-                           in _
-             ); eauto.
-  pose proof (value_inj _ _ _ _ Hva _ Hwa); subst. 
-  refine (let (Hab, Hincr2) := mk_node_correct (_ : wf env x2) H _ _ _ _ in _
-         ); eauto. 
-  split; destruct (env xa); eauto. 
-Qed.
-
-Lemma xorb_correct env bdd (Hwf: wf env bdd) n a b ab bdd' :
-  xorb bdd n a b = Some (ab, bdd') ->
-  forall va, value env bdd a va -> 
-  forall vb, value env bdd b vb -> 
-  (value env bdd' ab (Datatypes.xorb va vb)%bool * incr env bdd bdd').
-Proof.
-  revert bdd Hwf a b ab bdd'. 
-  induction n; intros bdd Hwf a b ab bdd' Hand va Hva vb Hvb. 
-  - discriminate. 
-  - simpl in Hand. 
-    Ltac s ::= 
-    repeat 
-      match goal with 
-        | |- context [(Datatypes.xorb _ false)%bool]  => rewrite Bool.xorb_false_r
-        | |- context [(Datatypes.xorb _ true)%bool]  => rewrite Bool.xorb_true_r
-        | |- context [(Datatypes.xorb false  _ )%bool]  => rewrite Bool.xorb_false_l
-        | |- context [(Datatypes.xorb true _ )%bool]  => rewrite Bool.xorb_true_l                   
-      end.
-  destruct a as [ | | a]; destruct b as [ | | b]; simpl in *; t s; eauto using negb_correct. 
+      + apply nat_compare_eq in Heq; subst; t s. 
+        eauto using binop_correct_eq. 
+      + t s; eauto using binop_correct_lt.
+        
+      + t s; eauto using binop_correct_gt. 
+  Qed.
   
-  destruct x as [[la xa] ha]. destruct x0 as [[lb xb] hb]. 
-  destruct (NPeano.Nat.compare xa xb) eqn: Heq.
-    + apply nat_compare_eq in Heq; subst; t s. 
-      eauto using binop_correct_eq. 
-    + t s; eauto using binop_correct_lt. 
-    + t s; eauto using binop_correct_gt. 
-Qed.
+  
+  Lemma orb_correct env bdd (Hwf: wf bdd) n a b ab bdd' :
+    orb bdd n a b = Some (ab, bdd') ->
+    forall va, value env bdd a va -> 
+          forall vb, value env bdd b vb -> 
+                (value env bdd' ab (va || vb)%bool * incr bdd bdd').
+  Proof.
+    revert bdd Hwf a b ab bdd'. 
+    induction n; intros bdd Hwf a b ab bdd' Hand va Hva vb Hvb. 
+    - discriminate. 
+    - simpl in Hand. 
+      Ltac s ::= 
+           try 
+           match goal with 
+             | |- context [(_ || false)%bool]  => rewrite Bool.orb_comm; simpl Datatypes.orb
+             | |- context [(_ || true)%bool]  => rewrite Bool.orb_comm; simpl  Datatypes.orb
+             | |- context [(false || _ )%bool]  => simpl  Datatypes.orb
+             | |- context [(true  || _ )%bool]  => simpl  Datatypes.orb
+           end.
+      destruct a as [ | | a]; destruct b as [ | | b]; simpl in *; t s.
+      destruct x as [[la xa] ha]. destruct x0 as [[lb xb] hb]. 
+      destruct (NPeano.Nat.compare xa xb) eqn: Heq.
+      + apply nat_compare_eq in Heq; subst; t s. 
+        eauto using binop_correct_eq. 
+      + t s; eauto using binop_correct_lt.        
+      + t s; eauto using binop_correct_gt.
+  Qed.  
+  
+  Lemma negb_correct env bdd (Hwf: wf bdd) n a a' bdd' :
+    negb bdd n a = Some (a', bdd') ->
+    forall va, value env bdd a va -> 
+          (value env bdd' a' (Datatypes.negb va)%bool * incr bdd bdd').
+  Proof.
+    revert bdd Hwf a a' bdd'. 
+    induction n; intros bdd Hwf a a' bdd' Hnegb va Hva. 
+    - discriminate. 
+    - simpl in Hnegb. 
+      Ltac s ::= 
+           try
+           match goal with 
+             | |- context [(Datatypes.negb false)%bool] =>  simpl Datatypes.negb 
+             | |- context [(Datatypes.negb true)%bool]  =>  simpl Datatypes.negb
+           end. 
+      destruct a as [ | | a]; simpl in *; t s.
+      destruct x as [[la xa] ha]; t s.
+      destruct (value_N_inversion env bdd a va Hva _ _ _ I) as [vla [vha [[Hla Hha] Hwa]]].
+      destruct (IHn _ Hwf _ _ _ I1 _ Hla) as [Hvx Hincr]; clear I1. 
+      refine (let (Hvx1,Hincr2) := IHn x0 (_ : wf x0) _ _ _ I0 
+                                       _ (_: value env _ ha vha) 
+              in _
+             ); eauto.
+      pose proof (value_inj _ _ _ _ Hva _ Hwa); subst. 
+      refine (let (Hab, Hincr2) := mk_node_correct (_ : wf x2) H _ _ _ _ in _
+             ); eauto. 
+      split; destruct (env xa); eauto. 
+  Qed.
+  
+  Lemma xorb_correct env bdd (Hwf: wf bdd) n a b ab bdd' :
+    xorb bdd n a b = Some (ab, bdd') ->
+    forall va, value env bdd a va -> 
+          forall vb, value env bdd b vb -> 
+                (value env bdd' ab (Datatypes.xorb va vb)%bool * incr bdd bdd').
+  Proof.
+    revert bdd Hwf a b ab bdd'. 
+    induction n; intros bdd Hwf a b ab bdd' Hand va Hva vb Hvb. 
+    - discriminate. 
+    - simpl in Hand. 
+      Ltac s ::= 
+           repeat 
+           match goal with 
+             | |- context [(Datatypes.xorb _ false)%bool]  => rewrite Bool.xorb_false_r
+             | |- context [(Datatypes.xorb _ true)%bool]  => rewrite Bool.xorb_true_r
+             | |- context [(Datatypes.xorb false  _ )%bool]  => rewrite Bool.xorb_false_l
+             | |- context [(Datatypes.xorb true _ )%bool]  => rewrite Bool.xorb_true_l                   
+           end.
+      destruct a as [ | | a]; destruct b as [ | | b]; simpl in *; t s; eauto using negb_correct. 
+      
+      destruct x as [[la xa] ha]. destruct x0 as [[lb xb] hb]. 
+      destruct (NPeano.Nat.compare xa xb) eqn: Heq.
+      + apply nat_compare_eq in Heq; subst; t s. 
+        eauto using binop_correct_eq. 
+      + t s; eauto using binop_correct_lt. 
+      + t s; eauto using binop_correct_gt. 
+  Qed.
+  
+ 
+  Lemma mk_var_correct env bdd (Hwf: wf bdd) v ptr bdd' :
+    mk_var bdd v = (ptr, bdd') -> 
+    value env bdd' ptr (env v) * incr bdd bdd'. 
+  Proof. 
+    unfold mk_var. intros. 
+    eapply (@mk_node_correct env) in H; eauto.  
+    destruct (env v); apply H. 
+  Qed. 
+  
 
-Lemma wf_expr env bdd (Hwf: wf env bdd) :forall p, (p < next bdd)%positive -> 
-                                              {vp : bool & value env bdd (N p) vp}.
+End value. 
+
+Inductive pvalue env bdd : expr -> bool -> Type :=
+| pvalue_T : pvalue env bdd T true
+| pvalue_F : pvalue env bdd F false
+| pvalue_N : forall (p : positive) (l : expr) (v : var) (h : expr),
+               PMap.find p (tmap bdd) = Some (l, v, h) ->
+               forall vl : bool,
+                 pvalue env bdd l vl ->
+                 forall vh : bool,
+                   pvalue env bdd h vh ->
+                   forall (r: bool), List.nth_error env v = Some r ->  
+                                pvalue env bdd (N p) (if r then vh else vl). 
+
+Hint Constructors pvalue. 
+
+Lemma list_nth_error_length {A} l (x: A):             
+       List.nth_error (l ++ [x]) (List.length l) = Some x. 
 Proof. 
-  intros. 
-  destruct (wf_lt_next_find env bdd Hwf p H) as [x Hx]. 
-  apply (wf_find_value env bdd Hwf p x Hx).
+  induction l. reflexivity. 
+  tauto. 
 Qed. 
 
-Definition ite bdd n c l r:=
-  do cl, bdd  <- andb bdd n c l;
-  do nc, bdd  <- negb bdd n c;
-  do ncr, bdd <- andb bdd n nc r;
-  orb bdd n cl ncr.
+Lemma pvalue_env_snoc bdd env x vx e : 
+  pvalue env bdd x vx -> 
+  pvalue (env ++ [e]) bdd x vx. 
+Proof. 
+  induction 1; auto. 
+  econstructor; eauto.  
+  Lemma list_nth_error_length_2 {A} l (x:A): 
+    forall v r, List.nth_error l v = Some r -> 
+         List.nth_error (l ++ [x]) v = Some r.  
+  Proof. 
+    induction l. 
+    destruct v; try discriminate.  
+    destruct v. simpl. tauto. 
+    intros. simpl. simpl in H. intuition. 
+  Qed. 
+  apply list_nth_error_length_2; auto. 
+Qed. 
+
+Lemma pvalue_incr bdd bdd' (Hincr: incr bdd bdd') env : 
+  forall x vx, 
+  pvalue env bdd x vx -> 
+  pvalue env bdd' x vx. 
+Proof. 
+  induction 1; auto. 
+  econstructor; eauto.  
+  apply Hincr. auto. 
+Qed. 
+
+Hint Resolve pvalue_incr. 
+Lemma pvalue_inj bdd env x vx:  
+  pvalue env bdd x vx -> 
+  forall vx' , pvalue env bdd x vx' -> 
+  vx = vx'. 
+Proof. 
+  induction 1. 
+  inversion 1. reflexivity. 
+  inversion 1; reflexivity. 
+  intros v2 Hv2. 
+  inversion Hv2. 
+  simpl in *. 
+  rewrite e in H2. inject H2. 
+  rewrite H5 in e0. inject e0. 
+  specialize (IHpvalue1 _ H3); clear H0 H3. 
+  specialize (IHpvalue2 _ H4); clear H H4. 
+  subst. reflexivity. 
+Qed. 
+
+Lemma pvalue_N_inversion :
+  forall env (bdd : BDD) (a : positive) (va : bool),
+    pvalue env bdd (N a) va ->
+    forall (l : expr) (x : var) (h : expr),
+      PMap.find a (tmap bdd) = Some (l, x, h) ->
+      forall vx, List.nth_error env x = Some vx -> 
+            {vl : bool &
+                       {vh : bool &
+                                  (pvalue env bdd l vl * pvalue env bdd h vh *
+                                   pvalue env bdd (N a) (if vx then vh else vl))%type}}. 
+Proof.   
+  intros. 
+  inversion H; subst. 
+  rewrite H0 in H3; inject H3. 
+  rewrite H1 in H6; inject H6. 
+  repeat eexists; eauto. 
+Qed. 
+
+Section pvalue. 
+  Lemma pvalue_upd  env bdd (Hwf: wf bdd) l v h:
+    NMap.find (l,v,h) (hmap bdd) = None ->
+    forall vl, pvalue env bdd l vl -> 
+          forall vh, pvalue env bdd h vh -> 
+                forall x vx, pvalue env bdd x vx -> 
+                        pvalue env (upd bdd (l,v,h)) x vx. 
+  Proof.              
+    intros Hbdd vl Hvl vh Hvh x vx H.
+    induction H. 
+    constructor. 
+    constructor. 
+    econstructor; eauto. 
+    simpl. rewrite PMap.gso. auto. 
+    destruct Hwf as [ _ Hwf]. apply Hwf in e. clear - e. zify; omega. 
+  Qed. 
+  Hint Resolve pvalue_upd.   
+
+  Lemma mk_node_pcorrect {env bdd} (Hwf: wf  bdd) {l v h e bdd'}: 
+    mk_node bdd l v h = (e,bdd') -> 
+    forall r, List.nth_error env v = Some r -> 
+    forall vl, pvalue env bdd l vl -> 
+          forall vh, pvalue env bdd h vh -> 
+                (pvalue env bdd' e (if r then vh else vl) * incr  bdd bdd')%type.       
+  Proof. 
+    intros.
+    unfold mk_node in H. 
+    case_eq (expr_eqb l h). 
+    - intros H'; rewrite H' in H. inject H.  
+      apply expr_eqb_correct in H'; subst. 
+      assert (vh = vl) by (eapply pvalue_inj; eauto); subst. 
+      destruct r;  split; eauto. 
+    - intros H'. rewrite H' in H.
+      case_eq (NMap.find (l,v,h) (hmap bdd)); [intros node Hnode | intros Hnode].
+    + rewrite Hnode in H.
+      injection H; intros; subst; clear H.
+      split ; [|auto]. 
+      rewrite (wf_bijection ) in Hnode. econstructor; eauto. 
+    + rewrite Hnode in H.
+      injection H; intros; subst; clear H.
+      assert (incr bdd (upd bdd (l,v,h))). 
+      {constructor.
+       * intros. 
+         simpl. rewrite PMap.gso; auto.  
+         apply wf_lt_next in H. zify;omega.         
+       * apply (order_upd); auto.  
+       * eapply path_upd; eauto.
+         Lemma path_of_pvalue env bdd x vx : 
+           pvalue env bdd x vx -> 
+           path bdd x. 
+         Proof. 
+           induction 1; try constructor. 
+           econstructor. apply e. auto.  auto. 
+         Qed. 
+         Hint Resolve path_of_pvalue. 
+ 
+         eauto. 
+         eauto. 
+       * intros. eapply wf_upd; eauto.  
+      }      
+      
+      { split; auto. 
+        intros.
+        econstructor;
+                [
+                | eapply pvalue_upd; eauto
+                | eapply pvalue_upd; eauto
+                | eauto].  
+        simpl. apply PMap.gss. 
+       }
+Qed.
+  Lemma pvalue_inv_env bdd env a va l x h :
+    PMap.find a (tmap bdd) = Some (l,x,h) -> 
+    pvalue env bdd (N a) va -> 
+    { vx |  List.nth_error env x = Some vx}. 
+  Proof. 
+    intros. 
+    inversion H0; subst. 
+    rewrite H in H2; inject H2. 
+    subst. eexists. apply H5.   
+  Qed. 
+  Hint Resolve pvalue_inv_env.
+  Section binop. 
+    Ltac inj :=
+      repeat match goal with 
+               | H : pvalue ?env ?b ?x ?vx , H' : pvalue ?env ?b  ?x ?vy |- _ =>  
+                 let H'' := fresh in 
+                 assert (H'' := pvalue_inj b env x vx H vy H'); 
+                   clear H'; subst
+             end. 
+    
+    Variables
+      (env : list bool)
+      (bdd : BDD)
+      (Hwf : wf bdd)
+      (op : bool -> bool -> bool)
+      (opb: BDD -> nat -> expr -> expr -> option (expr * BDD))
+      (n : nat)
+      (IH:  forall bdd : BDD,
+              wf  bdd ->
+              forall (a b ab : expr) (bdd' : BDD),
+                opb bdd n a b = Some (ab, bdd') ->
+              forall va : bool,
+                pvalue env bdd a va ->
+                forall vb : bool,
+                  pvalue env bdd b vb ->
+                  pvalue env bdd' ab (op va vb) * incr  bdd bdd')
+      (a b: positive)
+      (va vb: bool)
+      (Hva : pvalue env bdd (N a) va)
+      (Hvb : pvalue env bdd (N b) vb)
+      (la : expr) (xa: var) (ha: expr) (Ha : PMap.find a (tmap bdd) = Some (la, xa, ha)) 
+      (lb : expr) (xb: var) (hb: expr) (Hb : PMap.find b (tmap bdd) = Some (lb, xb, hb)).   
+  
+    Lemma binop_pcorrect_lt : forall
+                               l bdd1 (H1 : opb bdd n la (N b) = Some (l, bdd1))
+                               h bdd2 (H2 : opb bdd1 n ha (N b) = Some (h, bdd2))
+                               ab bdd3 (H3 : mk_node bdd2 l xa h = (ab, bdd3)),
+                               (pvalue env bdd3 ab (op va vb) * incr  bdd bdd3). 
+    Proof. 
+      intros. 
+      destruct (pvalue_inv_env _ _ _ _ _ _ _ Ha Hva) as [vxa Hxa]. 
+      destruct (pvalue_inv_env _ _ _ _ _ _ _ Hb Hvb) as [vxb Hxb]. 
+      destruct (pvalue_N_inversion env bdd a va Hva _ _ _ Ha _ Hxa) as [vla [vha [[Hla Hha] Hwa]]].
+      destruct (pvalue_N_inversion env bdd b vb Hvb _ _ _ Hb _ Hxb) as [vlb [vhb [[Hlb Hhb] Hwb]]].
+      destruct (IH _ Hwf _ _ _ _ H1 _ Hla _ Hwb) as [Hvx Hincr]. 
+      refine (let (Hvx1,Hincr2) := IH bdd1 (_ : wf  bdd1) _ _ _ _ H2 
+                                      _ (_: pvalue env bdd1 ha vha) 
+                                      _ (_: pvalue env bdd1 (N b) _) in _
+             ); eauto. 
+      inj. 
+      refine (let (Hab, Hincr2) := mk_node_pcorrect ( _ : wf bdd2) H3 _ _ _ _ _ _ in _
+             ); eauto. 
+      destruct (vxa); destruct (vxb); split; eauto.   
+    Qed. 
+    
+    Lemma binop_pcorrect_gt : forall
+                               l bdd1 (H1 : opb bdd n (N a) lb  = Some (l, bdd1))
+                               h bdd2 (H2 : opb bdd1 n (N a) hb = Some (h, bdd2))
+                               ab bdd3 (H3 : mk_node bdd2 l xb h = (ab, bdd3)),
+                               (pvalue env bdd3 ab (op va vb) * incr bdd bdd3). 
+    Proof. 
+      intros.  
+      destruct (pvalue_inv_env _ _ _ _ _ _ _ Ha Hva) as [vxa Hxa]. 
+      destruct (pvalue_inv_env _ _ _ _ _ _ _ Hb Hvb) as [vxb Hxb]. 
+      destruct (pvalue_N_inversion env bdd a va Hva _ _ _ Ha _ Hxa) as [vla [vha [[Hla Hha] Hwa]]].
+      destruct (pvalue_N_inversion env bdd b vb Hvb _ _ _ Hb _ Hxb) as [vlb [vhb [[Hlb Hhb] Hwb]]].
+      destruct (IH _ Hwf _ _ _ _ H1 _ Hwa _ Hlb) as [Hvx Hincr]. 
+      refine (let (Hvx1,Hincr2) := IH bdd1 (_ : wf  bdd1) _ _ _ _ H2 
+                                      _ (_: pvalue env bdd1 (N a) _) 
+                                      _ (_: pvalue env bdd1 hb vhb) in _
+             ); eauto. 
+      inj. 
+      refine (let (Hab, Hincr2) := mk_node_pcorrect ( _ : wf bdd2) H3 _ _ _ _ _ _ in _
+             ); eauto. 
+      destruct (vxa); destruct (vxb); split; eauto.  
+    Qed.
+  
+    Lemma binop_pcorrect_eq (Heq: xa = xb) : forall
+                                              l bdd1 (H1 : opb bdd n la lb  = Some (l, bdd1))
+                                              h bdd2 (H2 : opb bdd1 n ha hb = Some (h, bdd2))
+                                              ab bdd3 (H3 : mk_node bdd2 l xa h = (ab, bdd3)),
+                                              (pvalue env bdd3 ab (op va vb) * incr bdd bdd3). 
+    Proof. 
+      intros. 
+      destruct (pvalue_inv_env _ _ _ _ _ _ _ Ha Hva) as [vxa Hxa]. 
+      destruct (pvalue_inv_env _ _ _ _ _ _ _ Hb Hvb) as [vxb Hxb]. 
+      subst.  rewrite Hxb in Hxa; inject Hxa. 
+      destruct (pvalue_N_inversion env bdd a va Hva _ _ _ Ha _ Hxb) as [vla [vha [[Hla Hha] Hwa]]].
+      destruct (pvalue_N_inversion env bdd b vb Hvb _ _ _ Hb _ Hxb) as [vlb [vhb [[Hlb Hhb] Hwb]]].
+      destruct (IH _ Hwf _ _ _ _ H1 _ Hla _ Hlb) as [Hvx Hincr]. 
+      refine (let (Hvx1,Hincr2) := IH bdd1 (_ : wf bdd1) _ _ _ _ H2 
+                                      _ (_: pvalue env bdd1 ha vha) 
+                                      _ (_: pvalue env bdd1 hb vhb) in _
+             ); eauto. 
+      inj. 
+      refine (let (Hab, Hincr2) := mk_node_pcorrect _ H3 _ _ _ _ _ _  in _
+             ); eauto.
+      split; destruct (vxa); eauto.  
+    Qed. 
+  End binop.  
+
+  Ltac t s ::= 
+     repeat 
+     ((match goal with 
+       | H : Some _ = Some _ |- _ => injection H; clear H; intros; subst
+       | H : (None = Some _) |- _ => discriminate
+       | H : (bind ?F ?G = Some ?X) |- _ => 
+         destruct (bind_inversion _ _ F G _ H) as [?x [?I ?I]]; clear H
+       | H : (bind2 ?F ?G = Some ?X) |- _ => 
+         destruct (bind2_inversion F G _ H) as [?x [?x [?I ?I]]]; clear H
+       | |- context [(bind (Some _) ?G)] => simpl
+       | H : (bind ?x ?f = None) |- _ => 
+         destruct (bind_inversion_None x f H) as [?H | [?x [?I ?I]]]
+       | H : ?x = Some ?y |- context [?x] => rewrite H
+       | |- (_ * incr ?x ?x)%type => refine ( _ , incr_refl x )                              
+       | H : pvalue ?env ?b T _ |- _ => inversion_clear H
+       | H : pvalue ?env ?b F _ |- _ => inversion_clear H
+       | |- pvalue ?env _ T _ => constructor
+       | |- pvalue ?env _ F _ => constructor
+       | |- _ => subst           
+      end) || s); trivial.
+
+  Lemma andb_pcorrect env bdd (Hwf: wf bdd) n a b ab bdd' :
+    andb bdd n a b = Some (ab, bdd') ->
+    forall va, pvalue env bdd a va -> 
+          forall vb, pvalue env bdd b vb -> 
+                pvalue env bdd' ab (va && vb)%bool * incr bdd bdd'.
+  Proof.
+    revert bdd Hwf a b ab bdd'. 
+    induction n; intros bdd Hwf a b ab bdd' Hand va Hva vb Hvb. 
+    - discriminate. 
+    - simpl in Hand. 
+    Ltac s := 
+      try match goal with 
+            | |- context [(_ && false)%bool]  => rewrite Bool.andb_comm; simpl Datatypes.andb
+            | |- context [(_ && true)%bool]  => rewrite Bool.andb_comm; simpl  Datatypes.andb
+            | |- context [(false && _ )%bool]  => simpl  Datatypes.andb
+            | |- context [(true  && _ )%bool]  => simpl  Datatypes.andb
+          end.  
+    destruct a as [ | | a]; destruct b as [ | | b]; simpl in *; t s.   
+   
+    destruct x as [[la xa] ha]. destruct x0 as [[lb xb] hb]. 
+    destruct (NPeano.Nat.compare xa xb) eqn: Heq.
+      + apply nat_compare_eq in Heq; subst; t s.
+        eapply binop_pcorrect_eq; eauto.  
+      + t s; eauto using binop_pcorrect_lt.        
+      + t s; eauto using binop_pcorrect_gt. 
+  Qed.
+  
+  
+  Lemma orb_pcorrect env bdd (Hwf: wf bdd) n a b ab bdd' :
+    orb bdd n a b = Some (ab, bdd') ->
+    forall va, pvalue env bdd a va -> 
+          forall vb, pvalue env bdd b vb -> 
+                (pvalue env bdd' ab (va || vb)%bool * incr bdd bdd').
+  Proof.
+    revert bdd Hwf a b ab bdd'. 
+    induction n; intros bdd Hwf a b ab bdd' Hand va Hva vb Hvb. 
+    - discriminate. 
+    - simpl in Hand. 
+      Ltac s ::= 
+           try 
+           match goal with 
+             | |- context [(_ || false)%bool]  => rewrite Bool.orb_comm; simpl Datatypes.orb
+             | |- context [(_ || true)%bool]  => rewrite Bool.orb_comm; simpl  Datatypes.orb
+             | |- context [(false || _ )%bool]  => simpl  Datatypes.orb
+             | |- context [(true  || _ )%bool]  => simpl  Datatypes.orb
+           end.
+      destruct a as [ | | a]; destruct b as [ | | b]; simpl in *; t s.
+      destruct x as [[la xa] ha]. destruct x0 as [[lb xb] hb]. 
+      destruct (NPeano.Nat.compare xa xb) eqn: Heq.
+      + apply nat_compare_eq in Heq; subst; t s. 
+        eauto using binop_pcorrect_eq. 
+      + t s; eauto using binop_pcorrect_lt.        
+      + t s; eauto using binop_pcorrect_gt.
+  Qed.  
+  
+  Lemma negb_pcorrect env bdd (Hwf: wf bdd) n a a' bdd' :
+    negb bdd n a = Some (a', bdd') ->
+    forall va, pvalue env bdd a va -> 
+          (pvalue env bdd' a' (Datatypes.negb va)%bool * incr bdd bdd').
+  Proof.
+    revert bdd Hwf a a' bdd'. 
+    induction n; intros bdd Hwf a a' bdd' Hnegb va Hva. 
+    - discriminate. 
+    - simpl in Hnegb. 
+      Ltac s ::= 
+           try
+           match goal with 
+             | |- context [(Datatypes.negb false)%bool] =>  simpl Datatypes.negb 
+             | |- context [(Datatypes.negb true)%bool]  =>  simpl Datatypes.negb
+           end. 
+      destruct a as [ | | a]; simpl in *; t s.
+      destruct x as [[la xa] ha]; t s.
+      destruct (pvalue_inv_env _ _ _ _ _ _ _ I Hva) as [vxa Hxa]. 
+
+      destruct (pvalue_N_inversion env bdd a va Hva _ _ _ I _ Hxa) as [vla [vha [[Hla Hha] Hwa]]].
+      destruct (IHn _ Hwf _ _ _ I1 _ Hla) as [Hvx Hincr]; clear I1. 
+      refine (let (Hvx1,Hincr2) := IHn x0 (_ : wf x0) _ _ _ I0 
+                                       _ (_: pvalue env _ ha vha) 
+              in _
+             ); eauto.
+      pose proof (pvalue_inj _ _ _ _ Hva _ Hwa); subst. 
+      refine (let (Hab, Hincr2) := mk_node_pcorrect (_ : wf x2) H _ _ _ _ _ _ in _
+             ); eauto. 
+      split; destruct (vxa); eauto. 
+  Qed.
+  
+  Lemma xorb_pcorrect env bdd (Hwf: wf bdd) n a b ab bdd' :
+    xorb bdd n a b = Some (ab, bdd') ->
+    forall va, pvalue env bdd a va -> 
+          forall vb, pvalue env bdd b vb -> 
+                (pvalue env bdd' ab (Datatypes.xorb va vb)%bool * incr bdd bdd').
+  Proof.
+    revert bdd Hwf a b ab bdd'. 
+    induction n; intros bdd Hwf a b ab bdd' Hand va Hva vb Hvb. 
+    - discriminate. 
+    - simpl in Hand. 
+      Ltac s ::= 
+           repeat 
+           match goal with 
+             | |- context [(Datatypes.xorb _ false)%bool]  => rewrite Bool.xorb_false_r
+             | |- context [(Datatypes.xorb _ true)%bool]  => rewrite Bool.xorb_true_r
+             | |- context [(Datatypes.xorb false  _ )%bool]  => rewrite Bool.xorb_false_l
+             | |- context [(Datatypes.xorb true _ )%bool]  => rewrite Bool.xorb_true_l                   
+           end.
+      destruct a as [ | | a]; destruct b as [ | | b]; simpl in *; t s; eauto using negb_pcorrect. 
+      
+      destruct x as [[la xa] ha]. destruct x0 as [[lb xb] hb]. 
+      destruct (NPeano.Nat.compare xa xb) eqn: Heq.
+      + apply nat_compare_eq in Heq; subst; t s. 
+        eauto using binop_pcorrect_eq. 
+      + t s; eauto using binop_pcorrect_lt. 
+      + t s; eauto using binop_pcorrect_gt. 
+  Qed.
+   
+  Lemma mk_var_pcorrect' env bdd (Hwf: wf bdd) v ptr bdd' :
+    mk_var bdd v = (ptr, bdd') -> 
+    forall r, List.nth_error env v = Some r -> 
+    pvalue env bdd' ptr r * incr bdd bdd'. 
+  Proof. 
+    unfold mk_var. intros. 
+    eapply (@mk_node_pcorrect env) in H; eauto.  
+    destruct (r); apply H. 
+  Qed. 
+
+
+  Lemma mk_var_pcorrect bdd (Hwf: wf bdd) bdd' env ptr e: 
+    mk_var bdd (Datatypes.length env) = (ptr, bdd') -> 
+    pvalue (List.app env [e]) bdd' ptr e. 
+  Proof.   
+    intros. 
+    pose proof (mk_var_pcorrect' (List.app env [e]) _ _ _ _ _ H e).  
+    rewrite list_nth_error_length in X. specialize (X refl_equal). intuition.  
+  Qed. 
+
+  Lemma ite_pcorrect bdd (Hwf: wf bdd) bdd' n env c l r ptr: 
+    ite bdd n c l r = Some (ptr, bdd') -> 
+    forall vc, pvalue env bdd c vc -> 
+          forall vl, pvalue env bdd l vl -> 
+                forall vr, pvalue env bdd r vr -> 
+                      (pvalue env bdd' ptr  (if vc then vl else vr) * incr bdd bdd'). 
+  Proof. 
+    unfold ite.
+    intros H. simpl_do. intros. 
+    eapply andb_pcorrect in H0; eauto. destruct H0.      
+    eapply negb_pcorrect in H; eauto. destruct H.   
+    eapply andb_pcorrect in H1; eauto. destruct H1. 
+    eapply orb_pcorrect in H3; eauto. destruct H3. 
+    simpl in *. 
+    destruct vc; simpl in p2; split; eauto.   
+    rewrite Bool.orb_comm in p2. apply p2. 
+  Qed. 
+End pvalue. 
+
+Lemma mk_var_incr bdd (Hwf: wf bdd) bdd' n ptr: 
+  mk_var bdd n = (ptr, bdd') -> 
+  incr bdd bdd'. 
+Proof. 
+  intros. 
+  eapply (mk_var_correct (fun _ => false)) in H. 
+  destruct H. auto. 
+  auto. 
+Qed.   
+
+Lemma mk_var_path bdd bdd' (Hwf: wf bdd) n ptr: mk_var bdd n = (ptr, bdd') -> 
+                                  path bdd' ptr. 
+Proof. 
+  intros H. eapply (mk_var_correct (fun _ => false)) in H; auto.
+  destruct H as [Hv Hincr]. 
+  apply path_of_value in Hv. auto. 
+Qed. 
+
+
+
+Lemma wf_empty : wf empty. 
+Proof. 
+  constructor; simpl; intros.
+  - split; intro H. 
+    rewrite NMapFacts.empty_o in H. discriminate. 
+    rewrite PMap.gempty in H. discriminate. 
+  - rewrite PMap.gempty in H. discriminate.  
+  - exfalso. zify; omega. 
+  - exfalso. zify; omega. 
+  - inversion H. simpl in H1. rewrite PMap.gempty in H1. clear - H1; discriminate. 
+Qed. 
