src/CP.v
@@ -1,5 +1,5 @@
 Require Import Common DList Core ZArith. 
-Require BDD.
+Require BDD Seq.
 
 (* In this compilation pass, we implement boolean simplification using BDDs. *)
 
@@ -80,43 +80,49 @@ Section t.
   Record Env := mk
     {
       Ebdd : BDD.BDD;
-      Eknown: list (BDD.expr * Var Tbool);
+      
+      (* An association list that maps pointers in the BDD to variables *)
+      Eassoc: list (BDD.expr * Var Tbool);
+      
+      (* The denotation of the variables of the bdd (i.e, the uninterpreted booleans) *)
+      Evalues: list (Var Tbool); 
+      
       Enext: nat
     }. 
 
-  Definition empty : Env := mk BDD.empty [] 20. 
+  Definition empty : Env := mk BDD.empty [] [] 0. 
   
   Definition add_bdd (Gamma: Env) (b:bexpr ): option (BDD.expr * Env) :=  
     match b with
       | Lift x => Some (x, Gamma)
       | Ite c l r => 
           do v, bdd <- BDD.ite (Ebdd Gamma) (Enext Gamma) c l r;
-          Some (v, mk bdd (Eknown Gamma) (Enext Gamma))
+          Some (v, mk bdd (Eassoc Gamma) (Evalues Gamma) (Enext Gamma))
       | And a b => 
           do  r,bdd <- BDD.andb (Ebdd Gamma) (Enext Gamma) a b;
-          Some (r, mk bdd (Eknown Gamma) (Enext Gamma))
+          Some (r, mk bdd (Eassoc Gamma) (Evalues Gamma) (Enext Gamma))
       | Or a b => 
           do  r,bdd <- BDD.orb (Ebdd Gamma) (Enext Gamma) a b;
-          Some (r, mk bdd (Eknown Gamma) (Enext Gamma))
+          Some (r, mk bdd (Eassoc Gamma) (Evalues Gamma) (Enext Gamma))
       | Xor a b => 
           do r,bdd  <- BDD.xorb (Ebdd Gamma) (Enext Gamma) a b;
-          Some (r, mk bdd (Eknown Gamma) (Enext Gamma))
+          Some (r, mk bdd (Eassoc Gamma) (Evalues Gamma) (Enext Gamma))
       | Not a => 
           do r,bdd <- BDD.negb (Ebdd Gamma) (Enext Gamma) a;
-          Some (r, mk bdd (Eknown Gamma) (Enext Gamma))
+          Some (r, mk bdd (Eassoc Gamma) (Evalues Gamma) (Enext Gamma))
     end. 
 
   Definition lookup (Gamma: Env) (b: BDD.expr) : option (Var Tbool) :=
-    BDD.assoc BDD.expr_eqb b (Eknown Gamma). 
+    BDD.assoc BDD.expr_eqb b (Eassoc Gamma). 
 
-  Definition add_env (Gamma: Env) (v:Var Tbool) (b:BDD.expr): Env :=
-    mk (Ebdd Gamma) ((b,v) :: Eknown Gamma) (Enext Gamma). 
-  
-  Definition incr Gamma :=
+  Definition incr Gamma v :=
     let n := (Enext Gamma) in 
     let (r, bdd) := BDD.mk_var (Ebdd Gamma) n in
-      (r, mk bdd (Eknown Gamma) (S n)). 
+      (r, mk bdd (Eassoc Gamma) (Evalues Gamma ++ [v]) (S n)). 
 
+  Definition add_env (Gamma: Env) (v:Var Tbool) (b:BDD.expr): Env :=
+    mk (Ebdd Gamma) (List.app (Eassoc Gamma) [(b,v)]) (Evalues Gamma) (Enext Gamma). 
+  
   (* Unfortunately, multiple reads from the same state elements cannot be shared *)
   Fixpoint cp_telescope {A} (Gamma: Env) (T : telescope Phi V A) : telescope Phi Var A :=
     match T with
@@ -133,8 +139,7 @@ Section t.
                 fun cont e => 
                   (
                     k :- e; 
-                    let (ptr, Gamma) := incr Gamma in 
-                    let Gamma := add_env Gamma k ptr in (* we add the mapping ptr ~> k in the environment *)
+                    let (ptr, Gamma) := incr Gamma k in 
                     cp_telescope Gamma (cont (k, Some ptr))
                   )
               | Some v => 
@@ -183,156 +188,96 @@ Section t.
     (*            _ :- @Econstant  _ _ Tbool false ; *)
     (*            b) in  *)
     k :-- cp_telescope empty b;
-    match k with (v,g,e) =>
+   match k with (v,g,e) =>
                    & (fst v, fst g, cp_effects  e)
     end. 
 End t.   
+Arguments Ebdd {Var} e. 
+Arguments Evalues {Var} e. 
+Arguments Eassoc {Var} e. 
+Arguments Enext {Var} e. 
 
 Notation V := (fun t => eval_type t * sval)%type.   
 
-Definition lift (env : list (BDD.expr * bool)) : BDD.var -> bool :=
-  fun n => 
-    match List.nth_error env n with 
-      | None => true
-      | Some (e,b) => b
-    end. 
+  
+Definition value (E: Env eval_type) (e : BDD.expr) v :=
+  BDD.pvalue  (Evalues E) (Ebdd E) e v. 
 
-
-Definition interp (E: Env eval_type) v := 
-  BDD.interp (lift (Eknown _ E)) (Ebdd _ E) (S (Enext _ E)) v. 
-
-
-Definition eval_bexpr (E: Env eval_type) (b: bexpr) : option (bool) :=
-  match b with
-    | Lift x => interp E x 
-    | Ite c l r => do c <- interp E c; 
-                  do l <- interp E l;
-                  do r <- interp E r;
-                  Some (if c then l else r)
-    | And a b => do a <- interp E a; 
-                do b <- interp E b; 
-                Some (a && b)%bool
-    | Or a b => do a <- interp E a; 
-               do b <- interp E b; 
-               Some (a || b)%bool
-    | Xor a b => do a <- interp E a; 
-                do b <- interp E b; 
-                Some (xorb a b)%bool
-    | Not a => do a <- interp E a; 
-              Some (negb a)%bool
-  end. 
-
+Inductive bvalue (E: Env eval_type) : bexpr -> bool -> Type :=
+|bvalue_Lift: forall x vx, value E x vx -> 
+                     bvalue E (Lift x) vx 
+|bvalue_Ite: forall c vc, value E c vc -> 
+              forall l vl, value E l vl -> 
+              forall r vr, value E r vr -> 
+                     bvalue E (Ite c l r) (if vc then vl else vr)
+|bvalue_And: forall a va, value E a va -> 
+            forall b vb, value E b vb -> 
+                   bvalue E (And a b) (va && vb)
+|bvalue_Or: forall a va, value E a va -> 
+           forall b vb, value E b vb -> 
+                   bvalue E (Or a b) (va || vb)
+|bvalue_XOr: forall a va, value E a va -> 
+                     forall b vb, value E b vb -> 
+                  bvalue E (Xor a b) (xorb va vb)                         
+|bvalue_Not: forall a va, value E a va -> 
+                      bvalue E (Not a) (negb va). 
+    
 Notation "G |= x -- y" := (In _ _ _ x y G) (no associativity, at level 71). 
 
-Definition value (E: Env eval_type) sv x := match sv with 
-                                                None => False
-                                              | Some v => BDD.value (lift (Eknown _ E)) (Ebdd _ E) v x
-                                            end. 
+(* Recall that V t is defined as  eval_type t * sval, and sval = option BDD.expr. 
+   We have G |= x -- (v, Some e) when x = v and BDD.value e v 
+ *)
 
-
-  
-Class inv (G: Gamma eval_type V) (E: Env eval_type) :=
+Record inv (G: Gamma eval_type V) (E: Env eval_type) :=
   {
     inv_1 : forall t (x : eval_type t) y, G |= x -- y -> x = fst y;
-    inv_2 : forall (x: eval_type Tbool) y, G |= x -- y -> 
-                                      value E (snd y) x; 
-    inv_bdd_wf : BDD.wf (lift  (Eknown _ E)) (Ebdd _ E); 
-    inv_next : (Enext _ E) = BDD.wf_depth _ _ inv_bdd_wf
+    inv_2 : forall (x: eval_type Tbool) x' e , G |= x -- (x', Some e) -> 
+                                      value E e x; 
+    inv_path : forall  (x: eval_type B) x' e, G |= x -- (x',Some e) -> 
+                        BDD.path (Ebdd E) e;
+    inv_bdd_wf : BDD.wf  (Ebdd E); 
+    inv_next_2 : (Enext E) = List.length (Evalues E) ;
+    inv_assoc : forall x (y: BDD.expr), Seq.In (y,x) (Eassoc E) -> G |= x -- (x,Some y)            
   }. 
-    
-Lemma inv_interp {G E} {Hinv : inv G E} (x: eval_type Tbool) y e:
-  forall (H: G |= x -- (y, Some e)),  
-    interp E e = Some x. 
-Proof. 
-  intros. 
-  unfold interp. 
-  rewrite inv_next. apply BDD.interp_S.  apply BDD.wf_value_interp.  
-  apply inv_2 in H. simpl in H. apply H. 
-Qed. 
- 
+
+Arguments inv_1 {G E} _ t x y _.
+Arguments inv_2 {G E} _ x x' e _.
+Arguments inv_path {G E} _ x x' e _.
+Arguments inv_bdd_wf {G E} _.
+Arguments inv_next_2 {G E} _.
+Arguments inv_assoc {G E} _ x y _.
+
 Notation R := (fun G t x y => In _ _ t x y G).  
 
-(** The dependent type swiss-knife. *)
-Ltac t :=  subst; repeat match goal with 
-                       H : existT _ _ _ = existT _ _ _ |- _ => 
-                         apply Eqdep.EqdepTheory.inj_pair2 in H
-                   |   H : context [eq_rect ?t _ ?x ?t ?eq_refl] |- _ => 
-                         rewrite <- Eqdep.EqdepTheory.eq_rect_eq in H
-                   |   H : context [eq_rect ?t _ ?x ?t ?H'] |- _ => 
-                         rewrite (Eqdep.EqdepTheory.UIP_refl _ _ H') in H;
-                         rewrite <- Eqdep.EqdepTheory.eq_rect_eq in H
-                   |   H : existT _ ?t1 ?x1 = existT _ ?t2 ?x2 |- _ => 
-                         let H' := fresh "H'" in 
-                           apply EqdepFacts.eq_sigT_sig_eq in H; destruct H as [H H']; subst
-                         end; subst.
+Ltac d := 
+  repeat 
+    match goal with 
+          | x: (eval_type _ * sval)%type, 
+               H: _ |= _ -- ?x' |- _ => constr_eq x x'; destruct x
+          | H: context [snd ?x] |- _ => simpl in H
+          | H: ?x = Some _ |- _ => subst
+        end. 
 
-(* Lemma Gamma_inv_cons_bool G env e f sv :  *)
-(*   Gamma_inv G env -> *)
-(*   value env sv e ->  *)
-(*   forall (heq: e = f),  *)
-(*     Gamma_inv (cons eval_type V Tbool e (f,sv) G) env.  *)
-(* Proof.  *)
-(*   intros. constructor.  *)
-(*   - intros. inversion H0; t. reflexivity. apply Gamma_inv_1. eauto.  *)
-(*   - intros. admit.  *)
-(* Qed.  *)
-
-(* Lemma Gamma_inv_cons G env t e f:  *)
-(*   Gamma_inv G env -> *)
-(*   t <> Tbool ->  *)
-(*   forall  Heq : e = f,  *)
-(*     Gamma_inv (cons eval_type V t e (f,None) G) env.  *)
-(* Proof.  *)
-(*   intros. constructor.  *)
-(*   - intros. inversion H0; t. reflexivity. apply Gamma_inv_1. eauto.  *)
-(*   - intros. admit.  *)
-(* Qed.         *)
+Hint Unfold value.
 
 Lemma cp_expr_correct Phi st : 
-  forall t e1 r1, 
-    eval_expr Phi st t e1 = r1 ->
+  forall e1 r1, 
+    eval_expr Phi st B e1 = r1 ->
     forall G (env : Env eval_type) e2,
-      expr_equiv _ _ Phi (R G) t e1 e2 ->     
-      inv G env
-      -> match t as ty return eval_type ty -> Prop
-        with 
-          | Tbool => 
-            match snd (cp_expr Phi _ t  e2) 
-            with
-              | Some sv => fun r1 => eval_bexpr env sv  = Some r1
-              | None => fun _ => True
-            end
-          | _ => fun _ => True
-        end r1.
+      expr_equiv _ _ Phi (R G) B e1 e2 ->     
+      inv G env -> 
+      forall sv, snd (cp_expr Phi _ B  e2) = Some sv -> 
+            bvalue env sv r1. 
 Proof. 
-  destruct 1; inversion 1; t;  try solve [destruct t; simpl; auto]; intros. 
-  - simpl. destruct t; trivial; clear H. 
-    Require Import Equality. 
-
-    Ltac d :=
-      repeat match goal with 
-        | H : DList.pointwise _ (?t :: ?q) _ _ |- _ => 
-          apply DList.inversion_pointwise in H; 
-            destruct H
-        | H : DList.pointwise _  [] _ _ |- _ => clear H
-        | x :( _ * sval)%type |- _ => destruct x as [ ? [? | ]]
-      end. 
-
-    dependent destruction f; simpl; repeat DList.inversion; d; simpl; trivial;  
-    repeat match goal with 
-      | H :    ?G |= ?x -- (?v, Some ?e) |- context [?e] => 
-        rewrite (inv_interp _ _ _ H)
-    end; simpl; try reflexivity. 
-  - destruct t; trivial. destruct c; reflexivity.   
-  - destruct t; trivial; d;  simpl; trivial.  
-    repeat match goal with 
-             | H :    ?G |= ?x -- (?v, Some ?e) |- context [?e] => 
-               rewrite (inv_interp _ _ _ H)
-           end; simpl; try reflexivity. 
-  - trivial. 
-  - trivial. 
+  destruct 1; inversion 1; injectT;  try solve [destruct t; simpl; auto]; intros INV sv; simpl; try discriminate.  
+  - Require Import Equality. 
+    dependent destruction f; simpl; DList.inv; simpl;
+    intros; simpl_do; d; constructor; eapply inv_2; eassumption. 
+    Hint Constructors BDD.pvalue. 
+    Hint Constructors bvalue. 
+  - destruct c; simpl; intros H; inject H; eauto. 
+  - intros; simpl_do; d; constructor; eapply inv_2; eassumption. 
 Qed. 
-
 
 Lemma cp_effects_correct (Phi : state) st Delta G e  (Hg : inv G e):
   forall e1 e2 
@@ -344,19 +289,20 @@ Proof.
   apply DList.map3_map.   
   eapply DList.pointwise_map; [| apply H];
   clear H; simpl in *; intros. 
-  inversion H;  t; unfold RTL.R in *; 
+  inversion X; injectT; unfold RTL.R in *; 
   repeat (match goal with 
             | |- ?x = ?x  => reflexivity
             | |- context [match ?x with _=> _ end] => 
               case_eq x; intros
             | H' : In _ _ _ ?x ?y _ |- _ => 
-              rewrite (inv_1 _ _ _ H')
+              rewrite (inv_1 Hg _ _ _ H')
             | H : context [fst ?x] |- _ => progress (simpl in H)
             | H : ?x = ?x |- _ => clear H
             | H : ?y = ?x, H' : ?x = ?y |- _ => clear H'
             | x : (_ * _)%type |- _ =>  destruct x; simpl; subst
           end); simpl. 
-Qed. 
+Qed.
+ 
 Lemma inv_cons_None G E t e f: 
   inv G E -> 
   e = f -> 
@@ -364,12 +310,14 @@ Lemma inv_cons_None G E t e f:
 Proof. 
   intros Hinv Heq; subst. 
   econstructor. 
-  + intros.  
-    inversion H; t.  reflexivity. 
+  + intros ty x y.  inversion 1; injectT.  reflexivity. 
     apply Hinv; auto. 
     
-  + intros. admit. 
+  + intros x x' e H. inversion H; injectT. discriminate. eapply inv_2; eassumption.  
+  + intros x x' e H. inversion H; injectT. congruence.  eapply inv_path; eauto.  
   + apply Hinv. 
+  + intros. apply Hinv.
+  + intros. apply In_skip. eapply inv_assoc; eauto.  
 Qed. 
 
 Lemma cp_expr_correct_2 Phi st G env (Hg : inv G env) t:
@@ -379,32 +327,32 @@ Lemma cp_expr_correct_2 Phi st G env (Hg : inv G env) t:
 Proof.
   Ltac crush :=
     repeat (match goal with 
-      | H: (_,_) = (_,_) |- _ => injection H; clear H; intros; subst
+      | H: (_,_) = (_,_) |- _ => inject H
       | Hg : inv _ _ ,  H : In _ _ _ ?x ?y _ |- context [?x] =>
-        rewrite (inv_1 _ _ _ H)
+        rewrite (inv_1 Hg _ _ _ H)
       | H : DList.T [] |- _ => DList.inversion 
       | H : DList.T (_ :: _) |- _  => DList.inversion 
       | H : DList.pointwise _ ( _ :: _) _ _ |- _ => apply DList.inversion_pointwise in H; destruct H
     end); try reflexivity; try f_equal. 
-  intros e1. destruct e1; intros e2 H; inversion H; t; simpl; intros; unfold RTL.R in *; crush.
+  intros e1. destruct e1; intros e2 H; inversion H; injectT; simpl; intros; unfold RTL.R in *; crush.
   
   - simpl. f_equal. 
     clear H b. 
-    induction args; repeat DList.inversion;simpl; intuition. 
-    + crush.  eauto.  
+    induction args; DList.inv;simpl; intuition. 
+    + crush;  eauto. 
   -  destruct ty; crush. destruct c; crush. 
   - clear H.  
     destruct c2. simpl.  destruct s; simpl. destruct e3; simpl.
     
-    Ltac save :=
+    Ltac save Hg :=
       repeat match goal with 
         |  H : _ |= _ -- _ |- _ =>
-           pose proof (inv_1 _ _ _ H);
-           pose proof (inv_interp _ _ _ H);
+           pose proof (inv_1 Hg _ _ _ H);
+           pose proof (inv_2 Hg _ _ _ H);
                     clear H
       end. 
-    save. simpl in *; subst. compute in H0. injection H0; intros; subst. reflexivity. 
-    save. simpl in *; subst. compute in H0. injection H0; intros; subst. reflexivity.
+    save Hg. simpl in *; subst. inversion H0; reflexivity. 
+    save Hg. simpl in *; subst. inversion H0. reflexivity.    
     reflexivity. 
     reflexivity. 
   - simpl. clear H. 
@@ -414,11 +362,419 @@ Proof.
 Qed. 
 
 
+
+(* Lemma bdd_value_path bdd l e v:  *)
+(*   BDD.value (lift l) bdd e v ->  *)
+(*   BDD.path bdd (List.length l) e -> *)
+(*   (forall l' v', BDD.value (lift (l ++ l')) bdd e v' -> v' = v).  *)
+(* Proof.  *)
+(*   induction 1; intros. *)
+
+(*   inversion H0; t. tauto.   *)
+(*   inversion H0; t. tauto.   *)
+  
+(*   inversion H1; subst.  *)
+(*   assert ((l1,v0,h0) = (l0,v,h)) by congruence. *)
+(*   inject H3. clear H4.  *)
+(*   assert (IH1 := IHvalue1 H5).  *)
+(*   assert (IH2 := IHvalue2 H6). clear IHvalue1 IHvalue2 H5 H6.  *)
+(*   assert (H' := BDD.value_N_inversion _ _ _ _ H2 _ _ _ e).  *)
+(*   destruct H' as [vl2 [vh2 [[Hl'  Hv'  ] Hp' ]]].  *)
+(*   pose proof (BDD.value_inj _ _ _ _ H2 _ Hp' ).  *)
+(*   specialize (IH1 _ _ Hl'). specialize (IH2 _ _ Hv'). subst. *)
+(*   assert (lift (l++l') v = lift l v).  *)
+(*   clear - H7.  *)
+(*   apply lift_lt_length; auto.   *)
+(*   rewrite H3; congruence.  *)
+(* Qed.  *)
+
+(* Lemma bdd_value_lift_snoc bdd l ptr e x vx :  *)
+(*   BDD.value (lift l) bdd x vx ->  *)
+(*   BDD.path bdd (List.length l) x ->  *)
+(*   BDD.value (lift (l ++ [(ptr,e)])) bdd x vx.  *)
+(* Proof.  *)
+(*   intros.   *)
+(*   destruct (BDD.value_change_env _ (lift (l++ [(ptr,e)])) bdd _ _ H) as [vx' H'].  *)
+(*   assert (vx' = vx) by apply (bdd_value_path _ _ _ _ H H0 _ _ H').  *)
+(*   subst; auto.  *)
+(* Qed.  *)
+
+(* Arguments Eknown {Var} e.   *)
+(* Arguments Ebdd {Var} e.   *)
+(* Arguments Enext {Var} e.   *)
+Hint Resolve inv_bdd_wf.
+
+(* Lemma bdd_incr_path env bdd1 bdd2 n e (Hincr : BDD.incr env bdd1 bdd2):  *)
+(*   BDD.path bdd1 n e ->  *)
+(*   BDD.path bdd2 n e. *)
+(* Proof.  *)
+(* Admitted.  *)
+
+(* Lemma bdd_path_lt bdd n m e: n <= m ->  BDD.path bdd n e -> BDD.path bdd m e.  *)
+(* Proof.                *)
+(*   induction 2; try constructor.  *)
+(*   econstructor. eapply e. eauto. eauto.  *)
+(*   omega.  *)
+(* Qed.  *)
+   (* 
+Lemma inv_cons_incr G E (INV : inv G E) e ptr E2: 
+  incr eval_type E = (ptr, E2) -> 
+  inv (cons eval_type V B e (e, Some ptr) G) (add_env eval_type E2 e ptr).
+Proof. 
+  intros H. 
+  unfold incr in H. 
+  destruct (BDD.mk_var (Ebdd E) (Enext E)) as [r bdd] eqn:Heq. 
+  inject H. unfold add_env.  simpl. 
+  refine((fun Hwf => Build_inv _ _ _ _ _ Hwf (_) _ ) _). 
+  - intros ty x y; inversion 1; t.  reflexivity. 
+    apply INV; auto. 
+  - intros x y; inversion 1; t; simpl. 
+    {clear X. 
+     refine (let H := BDD.mk_var_correct (lift (Eknown E ++ [(ptr,e)])) _ _ _ _ _ Heq in _). 
+     eauto using BDD.wf_change_env.   
+     destruct H as [Hv Hincr]. 
+     assert (e = lift (Eknown E ++ [(ptr,e)]) (Enext E)) by 
+         (unfold lift; rewrite inv_next_2; rewrite list_nth_error_length; reflexivity). 
+     rewrite <- H in Hv. auto. }
+    {
+      destruct y as [y [?|]]. 
+      + pose proof (inv_2 _ _ X0). 
+        eapply BDD.mk_var_correct in Heq.
+        simpl in *. apply bdd_value_lift_snoc. 
+        eapply BDD.incr_value; [| apply H]. intuition eauto. 
+        eapply bdd_incr_path. 2: eapply inv_path. 2: eauto.  intuition eauto. 
+        eauto.      
+      + simpl. trivial. 
+    }
+  - intros x y z; inversion 1; t; simpl. 
+    inject H0. 
+    clear X. 
+    {    
+      unfold BDD.mk_var in Heq. unfold BDD.mk_node in Heq. simpl in Heq. 
+      destruct ( BDD.NMap.find (elt:=positive) (BDD.F, Enext E, BDD.T)
+                               (BDD.hmap (Ebdd E))) eqn:Heq'. 
+      
+      inject Heq.
+      econstructor. 
+      rewrite BDD.wf_bijection in Heq'. 
+      apply Heq'.
+      2: constructor. 
+      2: constructor. 
+      apply INV. 
+      rewrite inv_next_2.  rewrite List.app_length. simpl. omega. 
+      inject Heq.
+      econstructor. simpl. rewrite BDD.PMap.gss. reflexivity. 
+      constructor. 
+      constructor. 
+      rewrite inv_next_2.  rewrite List.app_length. simpl. omega. 
+      
+    }
+    {
+      
+    eapply bdd_path_lt. 
+    2: eapply bdd_incr_path. 3: eapply inv_path; eauto.  
+    rewrite List.app_length. simpl. omega. 
+    eapply BDD.mk_var_correct in Heq. 
+    destruct Heq; eauto. eauto. 
+    }
+  - simpl. simpl in *. 
+    unfold BDD.mk_var in Heq. unfold BDD.mk_node in Heq. 
+    simpl in Heq. 
+    destruct ( BDD.NMap.find (elt:=positive) (BDD.F, Enext E, BDD.T)
+            (BDD.hmap (Ebdd E))); inject Heq.  simpl. 
+    eapply BDD.mk_var_correct in Heq; eauto.  
+    destruct Heq as [Hv Hincr]. 
+    simpl in *. 
+  assert (BDD.wf (lift (Eknown eval_type E)) (Ebdd eval_type E))
+  econstructor. 
+  + intros ty x y; inversion 1; t.  reflexivity. 
+    apply INV; auto. 
+  + intros x y; inversion 1; t. 
+    {simpl. unfold incr in H. 
+     clear X. 
+     destruct (BDD.mk_var (Ebdd _ E) (Enext _ E)) as [r bdd] eqn:Heq. 
+     inject H. simpl. 
+     refine (let H :=
+                 BDD.mk_var_correct (lift (Eknown eval_type E ++ [(ptr,e)])) _ _ _ _ _ Heq
+             in _ ).   
+     eapply BDD.wf_change_env; apply INV.  
+     destruct H as [Hv Hi]. 
+     assert (e = lift (Eknown eval_type E ++ [(ptr,e)]) (Enext eval_type E)).
+     unfold lift. 
+     rewrite inv_next_2.
+     rewrite list_nth_error_length. reflexivity. 
+     rewrite <- H in Hv. auto. 
+    }
+    
+    {
+      destruct y as [y [?|]];
+      pose proof  (inv_2 _ _ X0);
+      trivial. 
+      pose proof (inv_path _ _ _ X0).             
+      unfold value in *; simpl in *.     
+      unfold incr in H. destruct (BDD.mk_var (Ebdd eval_type E) (Enext eval_type E)) eqn: Heq. 
+      inject H. simpl.
+      eapply BDD.mk_var_correct in Heq. 2: apply INV. 
+      
+      destruct Heq. 
+
+      apply bdd_value_lift_snoc; auto. 
+      apply i. auto. 
+      eapply bdd_incr_path. eauto. eauto. 
+    }
+  + intros x y z. inversion 1; t. inject H1. 
+    
+    {  
+      simpl. unfold incr in H. 
+      unfold incr in H. destruct (BDD.mk_var (Ebdd eval_type E) (Enext eval_type E)) eqn: Heq. 
+      inject H. simpl.
+      
+      
+      unfold BDD.mk_var in Heq. unfold BDD.mk_node in Heq. simpl in Heq. 
+      destruct ( BDD.NMap.find (elt:=positive) (BDD.F, Enext eval_type E, BDD.T)
+                               (BDD.hmap (Ebdd eval_type E))) eqn:Heq'. 
+      
+      inject Heq.  
+      econstructor. 
+      rewrite BDD.wf_bijection in Heq'. 
+      apply Heq'.
+      2: constructor. 
+      2: constructor. 
+      apply INV. 
+      rewrite inv_next_2.  rewrite List.app_length. simpl. omega. 
+      injection Heq. intros; subst. clear Heq.
+      econstructor. simpl. rewrite BDD.PMap.gss. reflexivity. 
+      constructor. 
+      constructor. 
+      rewrite inv_next_2.  rewrite List.app_length. simpl. omega. 
+    }
+    {
+      simpl. apply  inv_path in X0. 
+      Lemma incr_bdd_incr G E (INV : inv G E) ptr E2: 
+        incr eval_type E = (ptr, E2) -> 
+        BDD.incr (lift (Eknown _ E)) (Ebdd _ E) (Ebdd _ E2).   
+      Proof. 
+      Admitted. 
+      Hint Resolve incr_bdd_incr. 
+      Lemma incr_bdd_length_env G E (INV : inv G E) ptr E2: 
+        incr eval_type E = (ptr, E2) -> 
+        Datatypes.length (Eknown eval_type E) = Datatypes.length (Eknown  eval_type E2). 
+      Proof. 
+        unfold incr. destruct  (BDD.mk_var (Ebdd eval_type E) (Enext eval_type E)) eqn: Heq.
+        intros. injection H; clear H; intros; subst. simpl.  reflexivity. 
+      Qed. 
+      
+     
+      Hint Resolve bdd_path_lt.  Hint Resolve bdd_incr_path.
+      eauto. 
+      rewrite List.app_length. simpl. 
+      pose proof  (incr_bdd_length_env _ _ INV _ _ H). rewrite H0 in X0.  clear H0.
+      eapply bdd_path_lt.  
+      2: 
+        eapply bdd_incr_path. 3: apply X0. 2: eauto. simpl. 
+      generalize (Eknown eval_type E2). clear; intros; omega. 
+    }
+  + simpl.           
+    
+unfold incr in H. 
+          destruct  (BDD.mk_var (Ebdd eval_type E) (Enext eval_type E)) eqn: Heq.
+          injection H. intros; subst. clear H. simpl. 
+          simpl. 
+            2: eauto. 
+            econstructor. destruct INV.  
+            eapply BDD.mk_var_correct in Heq. 2: apply INV. 
+            
+          }
+          
+          {
+          }
+          }           simpl. 
+
+*)
+
+Lemma  incr_inv G E (INV : inv G E) ptr E' e : 
+  forall (H : incr eval_type E e = (ptr, E')), 
+    inv (cons eval_type V B e (e, Some ptr) G) E'. 
+Proof. 
+  intros H; unfold incr in H. 
+  destruct (BDD.mk_var (Ebdd E) (Enext E)) as [r bdd] eqn: Heq. 
+  inject H.
+  constructor. 
+  intros. 
+  - d. inversion X; injectT. inject H2. reflexivity. 
+    apply INV. auto. 
+  - intros x x' e'. inversion 1; injectT. clear X.
+    unfold value. inject H0. simpl.
+    eapply BDD.mk_var_pcorrect; eauto.  
+    erewrite <- inv_next_2; eauto. 
+    unfold value. simpl. 
+    eapply BDD.pvalue_env_snoc. eapply inv_2 in X0; eauto. eapply BDD.mk_var_incr in Heq; eauto.
+
+  - intros x x' e'. inversion 1; injectT. clear X. 
+    inject H0. simpl. 
+    eapply BDD.mk_var_path; eauto. 
+    simpl. 
+    eapply inv_path in X0;eauto. eapply BDD.mk_var_incr in Heq; eauto. 
+  - simpl. eapply BDD.mk_var_incr in Heq; eauto. 
+  - simpl. rewrite List.app_length. simpl. erewrite inv_next_2;eauto. rewrite plus_comm. reflexivity.
+  - simpl. intros x y H. apply In_skip. apply INV. auto.  
+Qed. 
+
+Lemma lookup_in E ptr x: 
+  lookup eval_type E ptr = Some x -> 
+  Seq.In (ptr,x) (Eassoc E). 
+Proof. 
+  unfold lookup. induction (Eassoc E). simpl. discriminate. 
+  simpl. destruct a.
+  destruct (BDD.expr_eqb ptr e) eqn: Heq. 
+  intros H; inject H.  
+  apply BDD.expr_eqb_correct in Heq; subst.
+  apply Seq.In_cons. 
+
+  intros H. right. auto. 
+Qed. 
+
+Lemma add_bdd_correct G E E' (INV: inv G E) sv v ptr: 
+  bvalue E sv v -> 
+  add_bdd eval_type E sv = Some (ptr, E') -> 
+  (value E' ptr v * inv G E' )%type. 
+Proof. 
+  destruct sv; simpl; intros H H'; simpl_do; inversion H; injectT.
+   
+  - split; eauto.  
+  - refine (let (Hv, Hi) := BDD.ite_pcorrect (Ebdd E) (inv_bdd_wf INV  : BDD.wf (Ebdd E))
+                                      _ _ _ c l r _ H0 _ H4 _ H6 _ H7 in _ ). 
+    split; eauto. 
+    Lemma inv_update_bdd G E bdd' (Hincr: BDD.incr (Ebdd E) bdd')
+    : inv G E -> 
+      inv G 
+          {| Ebdd := bdd'; 
+             Eassoc := Eassoc E; 
+             Evalues := Evalues E; 
+             Enext := Enext E|}. 
+      Proof. 
+        intros INV. constructor; try apply INV. 
+        simpl. intros. unfold value. simpl. eapply BDD.pvalue_incr; eauto. apply (inv_2 INV) in X; apply X.  
+        intros. simpl. eapply BDD.incr_path. eapply (inv_path INV) in X; apply X. 
+        simpl. apply Hincr. apply INV. 
+      Qed.         
+      apply inv_update_bdd; auto.  
+      
+  - refine (let (Hv,Hi) := BDD.andb_pcorrect (Evalues E) (Ebdd E) (inv_bdd_wf INV) _ _ _ _ x0 H0 va H3 vb H5 in _).
+    split; eauto using inv_update_bdd. 
+  - refine (let (Hv,Hi) := BDD.orb_pcorrect (Evalues E) (Ebdd E) (inv_bdd_wf INV) _ _ _ _ x0 H0 va H3 vb H5 in _).
+    split; auto using inv_update_bdd. 
+  - refine (let (Hv,Hi) := BDD.xorb_pcorrect (Evalues E) (Ebdd E)  (inv_bdd_wf INV) _ _ _ _ x0 H0 va H3 vb H5 in _).
+    split; auto using inv_update_bdd.     
+  - refine (let (Hv,Hi) := BDD.negb_pcorrect (Evalues E) (Ebdd E) (inv_bdd_wf INV) _ _ _  x0 H0 va H2 in _).
+    split; auto using inv_update_bdd. 
+Qed. 
+
+Lemma add_bdd_correct_2 G E E' (INV: inv G E) sv v ptr: 
+  bvalue E sv v -> 
+  add_bdd eval_type E sv = Some (ptr, E') -> 
+  forall x vx, 
+    value E x vx -> value E' x vx. 
+Proof. 
+  destruct sv; simpl; intros H H'; simpl_do; inversion H; injectT; clear H; auto. 
+  - refine (let (Hv, Hi) := BDD.ite_pcorrect (Ebdd E) (inv_bdd_wf INV : BDD.wf (Ebdd E))
+                                      _ _ _ c l r _ H0 _ H5 _ H7 _ H8 in _ ). 
+    eapply BDD.pvalue_incr. eauto.  simpl. eauto. 
+      
+  - refine (let (Hv,Hi) := BDD.andb_pcorrect (Evalues E) (Ebdd E) (inv_bdd_wf INV) _ _ _ _ x0 H0 va H4 vb H6 in _).
+    eauto using BDD.pvalue_incr. 
+  - refine (let (Hv,Hi) := BDD.orb_pcorrect (Evalues E) (Ebdd E) (inv_bdd_wf INV) _ _ _ _ x0 H0 va H4 vb H6 in _).
+    eauto using BDD.pvalue_incr. 
+  - refine (let (Hv,Hi) := BDD.xorb_pcorrect (Evalues E) (Ebdd E) (inv_bdd_wf INV) _ _ _ _ x0 H0 va H4 vb H6 in _).
+    eauto using BDD.pvalue_incr. 
+  - refine (let (Hv,Hi) := BDD.negb_pcorrect (Evalues E) (Ebdd E) (inv_bdd_wf INV) _ _ _  x0 H0 va H2 in _).
+    eauto using BDD.pvalue_incr. 
+Qed. 
+
+       
+Lemma inv_cons_lookup_Some G E (INV : inv G E) E2 sv ptr old v:
+  add_bdd eval_type E sv = Some (ptr, E2) -> 
+  lookup eval_type E2 ptr = Some old -> 
+  bvalue E sv v -> 
+  inv (cons eval_type V B v (old, Some ptr) G) E2. 
+Proof. 
+  intros. 
+  constructor. 
+  -intros.  d. inversion X; injectT. inject H5. clear X. 
+   simpl. 
+   
+   
+   apply lookup_in in H0. 
+   
+   destruct (add_bdd_correct _ _ _ INV _ _ _ H1 H) as [Hv INV2].  
+   apply (inv_assoc INV2) in H0. 
+   apply (inv_2 INV2) in H0. 
+   unfold value in *.           
+   eapply BDD.pvalue_inj; eauto. 
+   apply INV; auto. 
+  - intros x x' e. 
+    
+    inversion 1; injectT.
+    + clear X. inject H3. eapply add_bdd_correct in H; eauto.  intuition. 
+    + eapply add_bdd_correct_2; eauto.  
+      eapply inv_2 in X0; eauto. 
+  - intros x x' e. inversion 1; injectT.  inject H3. 
+    eapply add_bdd_correct in H; eauto.  destruct H as [Hv H'].
+    eapply BDD.path_of_pvalue; eauto.
+    
+    eapply (inv_path).  2: eapply X0.
+    eapply add_bdd_correct in H; eauto.  destruct H as [Hv H']. auto. 
+  - exact (let (_,H) := @add_bdd_correct _ _ _ INV _ _ _ H1 H in 
+           @inv_bdd_wf _ _ H). 
+  -  eapply add_bdd_correct in H; eauto.  destruct H as [Hv H']. apply H'.  
+  - intros.  eapply add_bdd_correct in H; eauto.  destruct H as [Hv H']. 
+    apply In_skip. apply H'. eauto.  
+Qed.
+
+Lemma inv_cons_lookup_None G E (INV : inv G E) E2 sv ptr X:
+  add_bdd eval_type E sv = Some (ptr, E2) -> 
+  lookup eval_type E2 ptr = None -> 
+  bvalue E sv X -> 
+  inv (cons eval_type V B X (X, Some ptr) G) (add_env eval_type E2 X ptr). 
+Proof. 
+  intros. 
+  constructor. 
+  -intros.  d. inversion X0; injectT. inject H5. reflexivity. 
+   eapply inv_1; eauto.     
+  - intros x x' e. inversion 1; injectT. inject H3.  
+    destruct (add_bdd_correct _ _ _ INV _ _ _ H1 H) as [Hv INV2].  
+    unfold add_env. 
+    unfold value. simpl. unfold value in Hv. apply Hv.
+    unfold value. simpl. 
+    eapply inv_2 in X1.
+    apply X1.     destruct (add_bdd_correct _ _ _ INV _ _ _ H1 H) as [Hv INV2].  eauto. 
+  - intros x x' e. inversion 1; injectT.  inject H3. 
+    eapply add_bdd_correct in H; eauto.  destruct H as [Hv H'].
+    eapply BDD.path_of_pvalue; eauto.
+
+    simpl. 
+    eapply (inv_path). 2: eapply X1.
+    eapply add_bdd_correct in H; eauto.  simpl. destruct H as [Hv H']. auto. 
+  - exact (let (_,H) := @add_bdd_correct _ _ _ INV _ _ _ H1 H in 
+           @inv_bdd_wf _ _ H). 
+  -  eapply add_bdd_correct in H; eauto.  destruct H as [Hv H']. apply H'.  
+  - intros. 
+    simpl in X0.
+    apply Seq.In_app in X0. 
+    eapply add_bdd_correct in H; eauto.  destruct H as [Hv H']. 
+    destruct X0. 
+    apply In_skip.    
+    apply H'.  auto. 
+    inversion i; subst. 
+    apply In_ok. reflexivity. reflexivity. 
+    inversion H2. 
+Qed. 
+
 Lemma cp_telescope_correct (Phi: state) st t  Delta: 
-     forall (b : RTL.block Phi eval_type t)
-       (b': RTL.block Phi V t)
-       (G : Gamma eval_type V),
-       block_equiv eval_type V Phi t G b b' ->
+       forall (b : RTL.block Phi eval_type t)
+         (b': RTL.block Phi V t)
+         (G : Gamma eval_type V),
+         block_equiv eval_type V Phi t G b b' ->
        forall e,
        inv  G e
      ->
@@ -437,8 +793,8 @@ Proof.
   Ltac crush ::=
     repeat match goal with 
              | H: (_,_) = (_,_) |- _ => injection H; clear H; intros; subst
-             | H : In _ _ _ ?x ?y _ |- context [?x] =>
-               rewrite (inv_1 _ _ _ H)
+             | HG : inv ?G ?e , H : In _ _ _ ?x ?y _ |- context [?x] =>
+               rewrite (inv_1 HG _ _ _ H)
              | H : DList.T [] |- _ => DList.inversion 
              | H : DList.T (_ :: _) |- _  => DList.inversion 
              | H : DList.pointwise _ ( _ :: _) _ _ |- _ => apply DList.inversion_pointwise in H; destruct H
@@ -463,50 +819,42 @@ Proof.
        destruct (lookup eval_type E2 ptr) as [old | ] eqn:Heq3; apply IH.
        clear IH. 
        pose proof (cp_expr_correct_2 _ st _ _ INV _ _ _ He _ _ Heq). 
-       rewrite H. 
-       pose proof (cp_expr_correct _ _ _ _ _ H _ _ _ He INV). simpl in H0.
-       rewrite Heq in H0. simpl in H0. 
-       Lemma inv_cons_lookup_Some G E (INV : inv G E) E2 sv ptr old X:
-         add_bdd eval_type E sv = Some (ptr, E2) -> 
-         lookup eval_type E2 ptr = Some old -> 
-         eval_bexpr E sv = Some X -> 
-         inv (cons eval_type V B X (old, Some ptr) G) E2. 
-       Proof. 
-       Admitted. 
-       eapply inv_cons_lookup_Some; eauto. 
+       rewrite H.
+       pose proof (cp_expr_correct _ _ _ _ H _ _ _ He INV sv). rewrite Heq in H0. simpl in H0. 
+       specialize (H0 eq_refl). 
+       eapply inv_cons_lookup_Some; eauto.  
        pose proof (cp_expr_correct_2 _ st _ _ INV _ _ _ He _ _ Heq). 
        rewrite H. 
-       pose proof (cp_expr_correct _ _ _ _ _ H _ _ _ He INV). simpl in H0.
-       rewrite Heq in H0. simpl in H0.
-       Lemma inv_cons_lookup_None G E (INV : inv G E) E2 sv ptr X:
-         add_bdd eval_type E sv = Some (ptr, E2) -> 
-         lookup eval_type E2 ptr = None -> 
-         eval_bexpr E sv = Some X -> 
-         inv (cons eval_type V B X (X, Some ptr) G) (add_env eval_type E2 X ptr). 
-       Proof. 
-       Admitted. 
+       pose proof (cp_expr_correct _ _ _ _ H _ _ _ He INV sv). simpl in H0.
+       rewrite Heq in H0. simpl in H0. specialize (H0 eq_refl). 
+
        eapply inv_cons_lookup_None; eauto. 
        apply inv_cons_None; eauto using cp_expr_correct_2. 
     }
     {
-      destruct (incr eval_type E) as [ptr E'] eqn: Hincr.
+      simpl. 
+      destruct (incr eval_type E (eval_expr Phi st B binding)) as [ptr E'] eqn: Hincr.
       apply IH; clear IH. 
       eapply cp_expr_correct_2 in Heq; eauto.  
       rewrite Heq; clear Heq.  
+      revert Hincr. 
       generalize (eval_expr Phi st B binding). 
-      intros e. 
-      Lemma inv_cons_incr G E (INV : inv G E) e ptr E2: 
-        incr eval_type E = (ptr, E2) -> 
-        inv (cons eval_type V B e (e, Some ptr) G) (add_env eval_type E2 e ptr).
-      Proof. 
-      Admitted. 
-      eapply inv_cons_incr; eauto. 
+      intros e H.
+      eapply incr_inv; eauto. 
     }
-Qed.     
+
+Qed.   
 
 Lemma Gamma_inv_empty : inv  (nil _ _ ) (empty eval_type). 
 Proof. 
-Admitted. 
+  econstructor. 
+  - intros. inversion X. 
+  - intros. inversion X. 
+  - intros. inversion X. 
+  - intros. apply BDD.wf_empty.  
+  - simpl. reflexivity. 
+  - simpl. intros.  inversion H. 
+Qed. 
 
 Theorem cp_correct Phi st t (b : Block Phi t) Delta : WF Phi t b -> 
   eval_block Phi st t (b _) Delta = eval_block Phi st t (cp_block Phi eval_type t (b _)) Delta. 
