src/CSE.v
@@ -13,19 +13,30 @@ Definition type_cast {P : type -> Type} {t} t' (x : P t) : option (P t') :=
           end) (type_eqb_correct t t' H)
    else fun _ => None) eq_refl. 
 
-(** The dependent type swiss-knife. *)
-Ltac t :=  subst; repeat match goal with 
-                       H : existT _ _ _ = existT _ _ _ |- _ => 
-                         apply Eqdep.EqdepTheory.inj_pair2 in H
-                   |   H : context [eq_rect ?t _ ?x ?t ?eq_refl] |- _ => 
-                         rewrite <- eq_rect_eq in H
-                   |   H : context [eq_rect ?t _ ?x ?t ?H'] |- _ => 
-                         rewrite (UIP_refl _ _ H') in H;
-                         rewrite <- eq_rect_eq in H
-                   |   H : existT _ ?t1 ?x1 = existT _ ?t2 ?x2 |- _ => 
-                         let H' := fresh "H'" in 
-                           apply eq_sigT_sig_eq in H; destruct H as [H H']; subst
-                         end; subst.
+Lemma type_cast_inversion t t' (x:eval_type t') (y: eval_type t) : type_cast t x = Some y -> 
+                                                                   t = t'. 
+Proof. 
+  unfold type_cast.
+  
+  generalize (type_eqb_correct t' t). simpl. pattern (type_eqb t' t). 
+  destruct (type_eqb t' t); try discriminate. 
+  intros e.
+  pose proof (e eq_refl). subst. reflexivity. 
+Qed. 
+
+(* (** The dependent type swiss-knife. *) *)
+(* Ltac t :=  subst; repeat match goal with  *)
+(*                        H : existT _ _ _ = existT _ _ _ |- _ =>  *)
+(*                          apply Eqdep.EqdepTheory.inj_pair2 in H *)
+(*                    |   H : context [eq_rect ?t _ ?x ?t ?eq_refl] |- _ =>  *)
+(*                          rewrite <- eq_rect_eq in H *)
+(*                    |   H : context [eq_rect ?t _ ?x ?t ?H'] |- _ =>  *)
+(*                          rewrite (UIP_refl _ _ H') in H; *)
+(*                          rewrite <- eq_rect_eq in H *)
+(*                    |   H : existT _ ?t1 ?x1 = existT _ ?t2 ?x2 |- _ => *)
+(*                        let H' := fresh "H'" in *)
+(*                          rewrite eq_sigT_iff_eq_dep in H; subst *)
+(*                          end; subst. *)
 
 Section s. 
   Variable Phi : state. 
@@ -221,7 +232,7 @@ Section s.
     
     
   
-  Definition Env := list ({t : type & (sval t * Var t)%type}). 
+  Definition Env : Type := list ({t : type & ((sval t * Var t) : Type )%type}). 
 
   Definition empty : Env := ([])%list. 
 
@@ -324,11 +335,12 @@ Notation R := (fun G t x y => In _ _ t x y G).
 Definition lift (env : Env eval_type) : list ({t : type & eval_type t}) :=
   List.map (fun x => match x with  existT t (sv,v) => existT _ t v end) env. 
 
+Require Seq. 
 Class Gamma_inv (G : Gamma eval_type V) (E : Env eval_type) :=
   {
     Gamma_inv_1 : forall t (x : eval_type t) y, G |= x -- y -> x = fst y;
     Gamma_inv_2 : forall t (x: eval_type t) y, G |= x -- y -> eval_sval (lift E) (snd y)  = Some x;
-    Gamma_inv_3 : forall t x sv, List.In (existT _ t (sv , x))  E -> G |= x -- (x,sv)
+    Gamma_inv_3 : forall t x sv, Seq.In (existT _ t (sv , x))  E -> G |= x -- (x,sv)
   }. 
  
 Hint Resolve Gamma_inv_1 Gamma_inv_2 Gamma_inv_3. 
@@ -416,7 +428,7 @@ Proof.
     simpl in *. rewrite Bool.andb_true_iff in H0. destruct H0.
     repeat f_equal. 
     destruct H. auto. 
-    destruct H. specialize (IHl _ H2 _ H1). clear - IHl. injection IHl; intros; t; auto. 
+    destruct H. specialize (IHl _ H2 _ H1). clear - IHl. injection IHl; intros; injectT; auto. 
   - pose proof (type_list_eqb_correct  _ _ H0); subst. 
     clear H0. 
     apply builtin_eqb_correct in H2; subst. 
@@ -436,8 +448,8 @@ Lemma cse_expr_correct : forall t e1 r1,
         | None => True
       end.
 Proof. 
-  destruct 1; inversion 1; t;  try solve [simpl; auto]; intros. 
-  - simpl. clear H. intro_do x Hx.  repeat f_equal.      
+  destruct 1; inversion 1; injectT;  try solve [simpl; auto]; intros. 
+  - simpl. clear X. intro_do x Hx.  repeat f_equal.      
     {
       revert Hx. clear f. 
       induction args; simpl; DList.inv. 
@@ -473,11 +485,11 @@ Proof.
     save. subst. simpl in *. DList.inv. simpl_do. auto. 
   - intros. simpl.  
     destruct dl2 as [hd tl]. simpl.  dependent destruction tl; try tauto.
-    clear H.
+    clear X.
     save; simpl in *; simpl_do; subst. 
 
     induction v; DList.inv; simpl in *; simpl_do; eauto.          
-  - simpl. repeat  use.  clear H.  
+  - simpl. repeat  use.  clear X.  
     induction l; DList.inv. 
     + reflexivity.
     + simpl in *.      
@@ -503,7 +515,7 @@ Qed.
 
 Lemma lookup_1 env t (sv : sval t) e :
   lookup eval_type t sv (env) = Some e ->
-  List.In (existT _ t (sv,e)) (env). 
+  Seq.In (existT _ t (sv,e)) (env). 
 Proof.
   intros. 
   induction env. discriminate.
@@ -512,23 +524,22 @@ Proof.
   pose proof (e0 eq_refl). subst. 
 
   case_eq (sval_eqb sv sv'); intros.    
-  left. t. rewrite H0 in H. 
-  repeat f_equal; try congruence || symmetry; auto using sval_eqb_correct. 
-  right.  apply IHenv. rewrite H0 in H.  auto. 
-  intros. 
-  simpl. right. auto. 
+  injectT. rewrite H0 in H.  apply sval_eqb_correct in H0. subst. inject H. apply Seq.In_cons. 
+  rewrite H0 in H. apply Seq.In_skip. auto. 
+  intros. apply Seq.In_skip.  auto. 
 Qed. 
 
 Lemma lem2  G env t e1 e2 sv : 
-  List.In (existT _ t (sv,e2)) (env) ->
+  Seq.In (existT _ t (sv,e2)) (env) ->
   Gamma_inv G env ->
   eval_sval  (lift env) sv = Some e1 ->
   G |= e1 -- (e2, sv). 
 Proof. 
   intros. 
-  apply (Gamma_inv_3 H0) in H. 
-  pose proof (Gamma_inv_2 H0 H). 
-  simpl in H2. 
+  
+  apply (Gamma_inv_3 X0) in X. 
+  pose proof (Gamma_inv_2 X0 X). 
+  simpl in H0. 
   
   assert ( e1 = e2). congruence.
   subst; auto. 
@@ -544,10 +555,10 @@ Proof.
   intros. 
   assert (eval_sval (lift env) sv = Some (eval_expr Phi st t e1)). eauto using lem1.
   
-  apply lookup_1 in H2.   
-  apply (Gamma_inv_3  H0) in H2. 
-  apply (Gamma_inv_2  H0) in H2. 
-  simpl in H2. congruence. 
+  apply lookup_1 in H0.   
+  apply (Gamma_inv_3  X0) in H0. 
+  apply (Gamma_inv_2  X0) in H0. 
+  simpl in *. congruence. 
 Qed. 
 
 Lemma Gamma_inv_cons G env t e sv : 
@@ -556,8 +567,8 @@ Lemma Gamma_inv_cons G env t e sv :
   Gamma_inv (cons eval_type V t e (e,sv) G) env. 
 Proof. 
   intros. constructor. 
-  - intros. inversion H1; t. reflexivity. eauto. 
-  - intros. inversion H1; t. simpl. eauto.  eauto. 
+  - intros ty x y. inversion 1;injectT. reflexivity. eauto. 
+  - intros ty x y. inversion 1;injectT. simpl. eauto.  eauto. 
   - intros. apply In_skip. eauto. 
 Qed. 
 
@@ -583,7 +594,7 @@ Proof.
       H': List.nth_error (?l ++ ?l') ?n = Some ?y |- _ =>
         pose proof (nth_error_app l l' n x H);
         assert (x = y) by congruence;
-        clear H H'; t; subst
+        clear H H'; subst
     | H : List.nth_error ?l ?n = Some ?x, 
       H': List.nth_error (?l ++ ?l') ?n = None |- _ =>
         pose proof (nth_error_app l l' n x H);
@@ -596,6 +607,9 @@ Proof.
   end;  auto || (try congruence) .
   induction sv using sval_ind_alt; simpl; intuition; crush.
 
+  injectT. 
+  simpl. 
+  auto. 
   - induction exprs; [intuition|inversion H; clear H];   intuition; crush. 
 
   - f_equal. clear f0. 
@@ -614,21 +628,17 @@ Proof.
 Qed. 
 
 
-Lemma list_in_snoc {A} l (x y : A) : List.In x (l++[y]) -> List.In x l \/  x = y. 
-Proof. 
-  revert x y. induction l. simpl; intuition.
-  simpl. intros x y [H | H]; auto. 
-  apply IHl in H. intuition.
-Qed. 
-  
-
 Lemma nth_error_map {A B} {f : A -> B} l t  :
   List.nth_error (List.map f (l ++ [t])) (List.length l) = Some (f t). 
 Proof. 
   induction l. reflexivity. 
   simpl. auto. 
-Qed. 
+Qed.
 
+(* Lemma list_in_snoc {} l (x y : A) : List.In x (l++[y]) -> ((List.In x l) + (x = y))%type.  *)
+(* Proof. *)
+(*   induction l. simpl; intuition. *)
+(* Admitted.    *)
 
 
 Lemma Gamma_inv_cons_var G env (Hg : Gamma_inv  G env) t (e : eval_type t): 
@@ -636,29 +646,28 @@ Lemma Gamma_inv_cons_var G env (Hg : Gamma_inv  G env) t (e : eval_type t):
                 (add eval_type t (SVar t (Datatypes.length env)) e env). 
 Proof.
   intros. 
-  constructor; intros. 
-  - inversion H; t. reflexivity.  use; reflexivity.  
-  - inversion H; t. simpl. unfold lift. unfold add. simpl. 
+  constructor.
+  - intros ty x y. inversion 1;injectT. reflexivity.  use; reflexivity.  
+  - intros ty x y. inversion 1;injectT. simpl. unfold lift. unfold add. simpl. 
     rewrite nth_error_map. simpl.
     
     apply type_cast_eq.
-    apply (Gamma_inv_2 Hg) in H1.
-    clear - H1. 
+    apply (Gamma_inv_2 Hg) in X0.
     unfold lift, add in *. 
 
     destruct y as [ y sv]. 
     rewrite List.map_app. 
-    revert H1. 
+    revert X0. clear X. 
     match goal with |- context [List.map ?f _] => set (F := f) end. 
     replace (List.length env) with (List.length (List.map F env)) by apply List.map_length.
     generalize (List.map F env).  intros. simpl. 
-    clear F. simpl in H1.  
+    clear F. simpl in X0.  
     apply eval_sval_monotone ; auto.    
     
     
-  - unfold add in H.  apply list_in_snoc in H. 
+  - intros ty x y H. unfold add in H.  apply Seq.In_app in H.  
     destruct H. apply In_skip. eauto. 
-    t. apply In_ok. congruence. congruence. 
+    inversion i. injectT. apply In_ok. congruence. congruence. inversion X. 
 Qed.         
       
 Lemma Gamma_inv_cons_other G env (Hg : Gamma_inv G env) t (e : eval_type t) sv: 
@@ -667,23 +676,23 @@ Lemma Gamma_inv_cons_other G env (Hg : Gamma_inv G env) t (e : eval_type t) sv:
             (add eval_type t sv e env). 
 Proof. 
   constructor. 
-  - intros. inversion H0; subst; t; subst. reflexivity.   eauto. 
-  - intros. inversion H0; subst; t; subst. 
+  - intros ty x y. inversion 1; subst; injectT; subst. reflexivity.   eauto. 
+  - intros ty x y. inversion 1; subst; injectT; subst. 
     simpl. unfold lift, add. rewrite List.map_app. apply eval_sval_monotone. apply H.
     simpl. unfold lift, add. rewrite List.map_app. apply eval_sval_monotone. eapply Gamma_inv_2; eauto. 
-  - intros.
-  unfold add in H0; apply list_in_snoc in H0. 
-  destruct H0. apply In_skip. eauto. 
-  t. apply In_ok. congruence. 
-  congruence. 
+  - intros ty x sv' H0.
+    unfold add in H0; apply Seq.In_app in H0. 
+    destruct H0. apply In_skip. eauto.
+    apply Seq.In_cons_inversion in i. destruct i. injectT. inject e0. apply In_ok; auto. 
+    apply Seq.In_nil in i; tauto. 
 Qed. 
 
 Lemma Gamma_inv_empty : Gamma_inv  (nil _ _ ) (empty eval_type). 
 Proof. 
-  constructor; intros. 
-  + inversion H. 
-  + inversion H. 
-  + simpl in H. tauto.  
+  constructor. 
+  + intros ty x y H; inversion H. 
+  + intros ty x y H; inversion H. 
+  + intros. simpl in X. apply Seq.In_nil in X. tauto. 
 Qed. 
 
 
@@ -700,14 +709,15 @@ Lemma cse_effects_correct (Phi : state) st Delta G e  (Hg : Gamma_inv Phi st G e
 Proof. 
   intros e1 e2 H.
   apply DList.map3_map. 
-  eapply DList.pointwise_map; [| apply H]. 
-  clear H;simpl; intuition. 
-  unfold R in *; inversion H; repeat t; simpl; clear H; trivial; destruct x3; try reflexivity.
-  rewrite (@Gamma_inv_1 _ _ _ _ Hg _ _ _ H4);
-  rewrite (@Gamma_inv_1 _ _ _ _ Hg _ _ _ H6); trivial. 
-  rewrite (@Gamma_inv_1 _ _ _ _ Hg _ _ _ H5);
-  rewrite (@Gamma_inv_1 _ _ _ _ Hg _ _ _ H6);
-  rewrite (@Gamma_inv_1 _ _ _ _ Hg _ _ _ H7); trivial. 
+  unfold effects_equiv in H. eapply DList.pointwise_map; [| apply H]. 
+  
+  clear H;simpl. intros t dt1 dt2 H v1 v2.  
+  unfold R in *; inversion H; injectT; simpl; clear H; trivial; destruct v2; try reflexivity.
+  rewrite (@Gamma_inv_1 _ _ _ _ Hg _ _ _ X);
+  rewrite (@Gamma_inv_1 _ _ _ _ Hg _ _ _ X0); trivial. 
+  rewrite (@Gamma_inv_1 _ _ _ _ Hg _ _ _ X);
+  rewrite (@Gamma_inv_1 _ _ _ _ Hg _ _ _ X0);
+  rewrite (@Gamma_inv_1 _ _ _ _ Hg _ _ _ X1); trivial. 
 Qed.  
 
 Lemma cse_expr_correct_2 Phi st G env (Hg : Gamma_inv Phi st G env) t:
@@ -724,7 +734,7 @@ Proof.
       | H : DList.T (_ :: _) |- _  => DList.inversion 
       | H : DList.pointwise _ ( _ :: _) _ _ |- _ => apply DList.inversion_pointwise in H; destruct H
     end); try reflexivity; try f_equal. 
-  intros e1. destruct e1; intros e2 H; inversion H; t; simpl; intros; unfold RTL.R in *; crush.
+  intros e1. destruct e1; intros e2 H; inversion H; injectT; simpl; intros; unfold RTL.R in *; crush.
   
   - simpl. f_equal. 
     clear dependent b. 
@@ -769,7 +779,7 @@ Lemma cse_telescope_correct (Phi: state) st t  Delta:
       (let (p, e0) := k in
        let (v, g) := p in & (fst v, fst g, cse_effects Phi eval_type e0))). 
 Proof. 
-  induction 1; simpl; intros. 
+  induction 1; simpl; intros E INV. 
   Ltac crush ::=
     repeat (match goal with 
       | H: (_,_) = (_,_) |- _ => injection H; clear H; intros; subst
@@ -788,22 +798,22 @@ Proof.
     crush. eauto using cse_effects_correct.  
   -  case_eq (cse_expr Phi eval_type a e2); intros; simpl.  
     + destruct o. 
-      case_eq (lookup Phi eval_type a s e0); intros; simpl; apply H; clear H.  
-      * assert (H' : eval_expr Phi st a e1 = e4) by eauto using lem1, lemma_2. 
+      case_eq (lookup Phi eval_type a s E); intros; simpl; apply H; clear H.  
+      * assert (H' : eval_expr Phi st a e1 = e3) by eauto using lem1, lemma_2. 
         rewrite H'. apply Gamma_inv_cons; auto. subst. eauto using lem1. 
-      * assert (H' : eval_expr Phi st a e1 = eval_expr Phi st a e3). 
+      * assert (H' : eval_expr Phi st a e1 = eval_expr Phi st a e0). 
         {
-          pose proof H1; eapply lem1 in H1; eauto. 
+          pose proof H0; eapply lem1 in H0; eauto. 
           eapply cse_expr_correct_2; eauto. }
         rewrite H'. 
-        assert (eval_sval Phi st (lift _ e0) s  = Some (eval_expr Phi st a e1)) by eauto using lem1. 
+        assert (eval_sval Phi st (lift _ E) s  = Some (eval_expr Phi st a e1)) by eauto using lem1. 
         apply Gamma_inv_cons_other; eauto.        
         congruence. 
       * apply H. clear H.   
-        assert (H' : eval_expr Phi st a e1 = eval_expr Phi st a e3) by 
+        assert (H' : eval_expr Phi st a e1 = eval_expr Phi st a e0) by 
                 (eauto using cse_expr_correct_2). 
          rewrite H' in *. 
-         generalize (eval_expr Phi st a e3); intros. 
+         generalize (eval_expr Phi st a e0); intros. 
          apply Gamma_inv_cons_var; auto.  
 Qed. 
 
@@ -824,3 +834,4 @@ Theorem Compile_correct Phi t b (Hwf : WF Phi t b): forall st Delta,
 Proof. 
   unfold Eval. intros. unfold Compile. symmetry. apply cse_correct. auto. 
 Qed. 
+
