src/Compiler.v
@@ -1,47 +1,53 @@
 Require Core Front IR RTL CSE CP FirstOrder (* DCE *). 
 
 
-Definition Compile Phi t  (a : forall Var, Front.action Phi Var t) : RTL.Block Phi t :=
+Definition front Phi t  (a : forall Var, Front.action Phi Var t) : RTL.Block Phi t :=
   let x := IR.Compile Phi  t a in
   let x := RTL.Compile Phi t x in 
   let x := CSE.Compile Phi t  x in  
         x. 
 
-Lemma Compile_correct (Phi : Core.state) t a :
-  let block := Compile Phi t a in 
-    RTL.WF Phi t (RTL.Compile _ _(IR.Compile _ _ a)) -> 
+Definition opt Phi t (x : RTL.Block Phi t) (* :  option (FirstOrder.block Phi t) *) :=
+  let x := CP.Compile Phi t x in
+    (* Constant propagation may have introduced some extra sharing,
+    and we may have to remove some occurences of Evar *)
+  let x := CSE.Compile Phi t x in
+  x. 
+
+Axiom HWF : forall Phi t p, RTL.WF Phi t p. 
+Lemma front_correct (Phi : Core.state) t a :
+  let block := front Phi t a in 
   forall st Delta, 
     RTL.Eval Phi st t block Delta =
     Front.Eval Phi st t a Delta. 
 Proof.
-  unfold Compile. intros. 
+  unfold front. intros. 
   rewrite CSE.Compile_correct. 
   rewrite RTL.Compile_correct. 
   rewrite IR.Compile_correct. 
   reflexivity. 
-  apply H. 
+  apply HWF. 
 Qed. 
 
-Print Assumptions Compile_correct. 
+Lemma opt_correct (Phi : Core.state) t src :
+  let tgt := opt _ _ src in 
+  forall st Delta, 
+    RTL.Eval Phi st t tgt Delta =
+    RTL.Eval Phi st t src Delta. 
+Proof. 
+  unfold opt; intros. 
+  rewrite CSE.Compile_correct by apply HWF.  
+  rewrite CP.Compile_correct by apply HWF.  
+  reflexivity. 
+Qed.   
 
-Definition Fo_compile Phi t (A : Front.Action Phi t) :=
-  let x := Compile Phi t A in 
-    FirstOrder.compile Phi t (x _ ).  
-
-
-Definition Fo_CP_compile Phi t (A : Front.Action Phi t) :=
-  let x := Compile Phi t A in 
-  let x := CP.Compile Phi t x in 
-    (* Constant propagation may have introduced some extra sharing,
-    and we may have to remove some occurences of Evar *)
-  let x := CSE.Compile Phi t x in 
-    FirstOrder.compile Phi t (x _ ).  
-
-Definition copt Phi t (A : Front.Action Phi t) (* :  option (FirstOrder.block Phi t) *) :=
-  let x := Compile Phi t A in 
-  (* let x := CP.Compile Phi t x in  *)
-    (* Constant propagation may have introduced some extra sharing,
-    and we may have to remove some occurences of Evar *)
-  (* let x := CSE.Compile Phi t x in  *)
+Definition fesic Phi t src := 
+  let x := (front Phi t src) in 
   let x := FirstOrder.compile Phi t (x _ ) in 
-    (* DCE.compile Phi   *) Some x.
+  (* DCE.compile Phi   *) Some x.
+ 
+Definition fesiopt Phi t x := 
+  let x := opt Phi t (front Phi t x) in 
+  let x := FirstOrder.compile Phi t (x _ ) in 
+  (* DCE.compile Phi   *) Some x.
+
